Gvf_Agent_Specification.thy
@@ -13,6 +13,15 @@ theory Gvf_Agent_Specification imports Gvf_Hoare_Logic begin
 type_synonym ht_specification = \<open>(Bcap \<times> \<Phi>\<^sub>M \<times> hoare_triple list) list\<close>
 \<comment> \<open>Set of pairs of mental state formula (enabled) and set of Hoare triple axioms.\<close>
 
+\<comment> \<open>Specify and insert invariants into a specification.\<close>
+fun add_invariant :: \<open>\<Phi>\<^sub>M \<Rightarrow> ht_specification \<Rightarrow> ht_specification\<close> where
+  \<open>add_invariant h [] = []\<close> |
+  \<open>add_invariant h ((a, \<Phi>, hts) # S') = (a, \<Phi>, \<^bold>{ h \<^bold>} (basic a) \<^bold>{ h \<^bold>} # hts) # add_invariant h S'\<close>
+
+fun add_invariants :: \<open>ht_specification \<Rightarrow> \<Phi>\<^sub>M list \<Rightarrow> ht_specification\<close> where
+  \<open>add_invariants S [] = S\<close> |
+  \<open>add_invariants S (h # t) = add_invariants (add_invariant h S) t\<close>
+
 section \<open>Satisfiability of specification\<close>
 
 \<comment> \<open>The main idea behind this, and the following, section is that we now base agents on specifications.
@@ -20,37 +29,29 @@ section \<open>Satisfiability of specification\<close>
     a link between agent specification and belief update function. We can reduce this problem to the
     problem of proving the existence of a belief update function (model) given a specification.\<close>
 
-\<comment> \<open>Satisfiability of a specification.\<close>
-definition satisfiable :: \<open>ht_specification \<Rightarrow> bool\<close> where
-  \<open>satisfiable S \<equiv> 
-    \<comment> \<open>Quantify over all mental states. Go through each element s in S.\<close>
-    \<forall>M. \<forall>s \<in> set S. 
-      \<comment> \<open>Get fields in s. Define a variable for the set of preconditions satisfied by M.\<close>
-      (let (_, \<Phi>, hts) = s; sat_hts = { ht \<in> set hts. M \<Turnstile>\<^sub>M pre ht } in
-        \<comment> \<open>If the basic action is enabled (\<Phi>)\<close>
-        (M \<Turnstile>\<^sub>M \<Phi> \<longrightarrow> 
-          \<comment> \<open>There exists a mental state M'...\<close>
-          (\<exists>M'. 
-            \<comment> \<open>That preserves consistency, and ...\<close>
-            (\<not> fst M \<Turnstile>\<^sub>L \<bottom>\<^sub>L \<longrightarrow> \<not> fst M' \<Turnstile>\<^sub>L \<bottom>\<^sub>L) \<and> 
-            \<comment> \<open>Where the goal base is obtained by removing achieved goals, and ...\<close>
-            (snd M' = snd M - {\<psi> \<in> snd M. fst M' \<Turnstile>\<^sub>L \<psi>}) \<and> 
-            \<comment> \<open>That satisfy all of the Hoare triples for this basic action.\<close>
-            (\<forall>ht \<in> sat_hts. M' \<Turnstile>\<^sub>M post ht))) \<and>
-        \<comment> \<open>If the basic action is not enabled, the Hoare triples should be satisfied by M.\<close>
-        (M \<Turnstile>\<^sub>M \<^bold>\<not> \<Phi> \<longrightarrow> (\<forall>ht \<in> sat_hts. M \<Turnstile>\<^sub>M post ht)))\<close>
+definition satisfiable_base :: \<open>mental_state \<Rightarrow> hoare_triple list \<Rightarrow> \<Phi>\<^sub>L set \<Rightarrow> bool\<close> where
+  \<open>satisfiable_base M hts \<Sigma> \<equiv>
+    (\<not> fst M \<^bold>\<Turnstile>\<^sub>P \<^bold>\<bottom> \<longrightarrow> \<not> \<Sigma> \<^bold>\<Turnstile>\<^sub>P \<^bold>\<bottom>) \<and> 
+    (\<forall>ht \<in> set hts. M \<Turnstile>\<^sub>M pre ht \<longrightarrow> (\<Sigma>, snd M - {\<psi> \<in> snd M. \<Sigma> \<^bold>\<Turnstile>\<^sub>P \<psi>} ) \<Turnstile>\<^sub>M post ht)\<close>
 
+definition satisfiable_elem :: \<open>mental_state \<Rightarrow> (Bcap \<times> \<Phi>\<^sub>M \<times> hoare_triple list) \<Rightarrow> bool\<close> where
+ \<open>satisfiable_elem M s \<equiv> 
+    (M \<Turnstile>\<^sub>M fst (snd s) \<longrightarrow> (\<exists> \<Sigma>. satisfiable_base M (snd (snd s)) \<Sigma>)) \<and> 
+    (M \<Turnstile>\<^sub>M \<^bold>\<not> (fst (snd s)) \<longrightarrow> (\<forall>ht \<in> set (snd (snd s)). M \<Turnstile>\<^sub>M pre ht \<longrightarrow> M \<Turnstile>\<^sub>M post ht))\<close>
+
+definition satisfiable :: \<open>ht_specification \<Rightarrow> bool\<close> where
+  \<open>satisfiable S \<equiv>  \<forall>M. \<forall>s \<in> set S. satisfiable_elem M s\<close>
 
 \<comment> \<open>We restrict those elements of the type 'ht_specification' that are valid specifications.\<close>
 \<comment> \<open>Hoare triples only for basic actions and should be for grouped for actions.\<close>
 fun is_ht_specification_hts :: \<open>Bcap \<Rightarrow> hoare_triple list \<Rightarrow> bool\<close>  where
   \<open>is_ht_specification_hts n hts = 
-    (\<forall>ht\<in> set hts. is_htb_basic ht \<and> fst (snd (the (htb_basic_unpack ht))) = n)\<close>
+    (hts \<noteq> [] \<and> (\<forall>ht\<in> set hts. is_htb_basic ht \<and> fst (snd (the (htb_basic_unpack ht))) = n))\<close>
 
 \<comment> \<open>Main definition. Each action (group) can only appear once, S is satisfiable and each element
    s of S satisfy the function defined above.\<close>
 definition is_ht_specification :: \<open>ht_specification \<Rightarrow> bool\<close> where
-  \<open>is_ht_specification S \<equiv> distinct (map fst S) \<and> satisfiable S \<and> 
+  \<open>is_ht_specification S \<equiv> S \<noteq> [] \<and> distinct (map fst S) \<and> satisfiable S \<and> 
                             (\<forall>s \<in> set S. is_ht_specification_hts (fst s) (snd (snd s)))\<close>
 
 \<comment> \<open>State that a given \<T> complies to our assumptions, partly due to semantics of Hoare triples
@@ -60,7 +61,7 @@ fun complies_ht :: \<open>mental_state \<Rightarrow> bel_upd_t \<Rightarrow> \<P
     \<comment> \<open>\<Phi> specify if the action is enabled\<close>
     ((M \<Turnstile>\<^sub>M \<Phi> \<longleftrightarrow> \<T> n M \<noteq> None) \<and>
     \<comment> \<open>Transitions preserves consistency.\<close>
-    (\<not> (fst M) \<Turnstile>\<^sub>L \<bottom>\<^sub>L \<longrightarrow> \<T> n M \<noteq> None \<longrightarrow> \<not>the (\<T> n M) \<Turnstile>\<^sub>L \<bottom>\<^sub>L) \<and>
+    (\<not> (fst M) \<^bold>\<Turnstile>\<^sub>P \<^bold>\<bottom> \<longrightarrow> \<T> n M \<noteq> None \<longrightarrow> \<not>the (\<T> n M) \<^bold>\<Turnstile>\<^sub>P \<^bold>\<bottom>) \<and>
     \<comment> \<open>Basic Hoare triple semantics for action enabled.\<close>
     (M \<Turnstile>\<^sub>M \<phi> \<and> M \<Turnstile>\<^sub>M \<Phi> \<longrightarrow> the (\<M>* \<T> (basic n) M) \<Turnstile>\<^sub>M \<psi>) \<and>
     \<comment> \<open>Basic Hoare triple semantics for action not enabled.\<close>
@@ -78,7 +79,7 @@ definition complies_hts :: \<open>(Bcap \<times> \<Phi>\<^sub>M \<times> hoare_t
 
 \<comment> \<open>Main definition. Does the specification comply to a given belief update function?\<close>
 definition complies :: \<open>ht_specification \<Rightarrow> bel_upd_t \<Rightarrow> bool\<close> where
-  \<open>complies S \<T> \<equiv> (\<forall>s\<in>set S. complies_hts s \<T> \<and> (\<forall>n. n \<notin> set (map fst S) \<longrightarrow> (\<forall>M. \<T> n M = None)))\<close>
+  \<open>complies S \<T> \<equiv> (\<forall>s\<in>set S. complies_hts s \<T>) \<and> (\<forall>n. n \<notin> set (map fst S) \<longrightarrow> (\<forall>M. \<T> n M = None))\<close>
 
 section \<open>Model existence\<close>
 
@@ -92,75 +93,72 @@ proof
   let ?\<T> = \<open>\<lambda>n. if n \<in> set (map fst S) then (SOME \<T>. complies_hts (THE s'. s'\<in>set S \<and> n = fst s') \<T>) n else (\<lambda>M. None)\<close>
   show \<open>complies S ?\<T>\<close> unfolding complies_def 
   proof
-    fix s   
-    assume member: \<open>s \<in> set S\<close>
-    have \<open>complies_hts s ?\<T>\<close>    
-    proof (cases s)
-      case f1: (fields n \<Phi> hts)
-      have \<open>\<forall>ht\<in>set hts. \<forall>M. complies_ht M ?\<T> \<Phi> (the (htb_basic_unpack ht))\<close>
-      proof
-        fix ht
-        assume \<open>ht \<in> set hts\<close>
-        show \<open>\<forall>M. complies_ht M ?\<T> \<Phi> (the (htb_basic_unpack ht))\<close>
+    show \<open>\<forall>s\<in>set S. complies_hts s ?\<T>\<close>
+    proof
+      fix s   
+      assume member: \<open>s \<in> set S\<close>
+      show \<open>complies_hts s ?\<T>\<close>    
+      proof (cases s)
+        case f1: (fields n \<Phi> hts)
+        have \<open>\<forall>ht\<in>set hts. \<forall>M. complies_ht M ?\<T> \<Phi> (the (htb_basic_unpack ht))\<close>
         proof
-          fix M
-          show \<open>complies_ht M ?\<T> \<Phi> (the (htb_basic_unpack ht))\<close>
-          proof (cases \<open>(the (htb_basic_unpack ht))\<close>)
-            case (fields \<phi> n' \<psi>)
-            have \<open>s\<in>set S \<and> fst s = fst s\<close> using \<open>s \<in> set S\<close> by simp
-            moreover have \<open>\<forall>s'. s'\<in>set S \<and> fst s = fst s' \<longrightarrow> s' = s\<close> using \<open>distinct (map fst S)\<close>
-              by (metis member eq_key_imp_eq_value prod.collapse)
-            ultimately have \<open>(THE s'. s'\<in>set S \<and> fst s = fst s') = s\<close> using the_equality by auto
-            then have \<open>?\<T> (fst s) = (SOME \<T>. complies_hts s \<T>) (fst s)\<close> (is \<open>?\<T> (fst s) = ?\<T>' (fst s)\<close>) using member by simp
-            have \<open>\<exists>\<T>. complies_hts s \<T>\<close> using assms(2) member by simp
-            then have \<open>complies_hts s ?\<T>'\<close> using someI_ex[where ?P=\<open>complies_hts s\<close>] by simp
-            then have \<open>\<forall>ht\<in>set hts. is_htb_basic ht \<and> (\<forall>M. complies_ht M ?\<T>' \<Phi> (the (htb_basic_unpack ht)))\<close> 
-              using f1 complies_hts_def by fastforce
-            with f1 \<open>ht \<in> set hts\<close> have \<open>\<forall>M. complies_ht M ?\<T>' \<Phi> (the (htb_basic_unpack ht))\<close> by simp
-            then have \<open>complies_ht M ?\<T>' \<Phi> (the (htb_basic_unpack ht))\<close> by blast
-            moreover have \<open>n = n'\<close> 
-              using fields assms(1) f1 member \<open>ht \<in> set hts\<close> unfolding is_ht_specification_def by fastforce
-            ultimately have \<open>complies_ht M ?\<T>' \<Phi> (\<phi>, n, \<psi>)\<close> using fields by simp
-            then have 
-              \<open>(M \<Turnstile>\<^sub>M \<Phi> \<longleftrightarrow> ?\<T>' n M \<noteq> None) \<and>
-              (\<not> (fst M) \<Turnstile>\<^sub>L \<bottom>\<^sub>L \<longrightarrow> ?\<T>' n M \<noteq> None \<longrightarrow> \<not>the (?\<T>' n M) \<Turnstile>\<^sub>L \<bottom>\<^sub>L) \<and>
-              (M \<Turnstile>\<^sub>M \<phi> \<and> M \<Turnstile>\<^sub>M \<Phi> \<longrightarrow> the (\<M>* ?\<T>' (basic n) M) \<Turnstile>\<^sub>M \<psi>) \<and>
-              (M \<Turnstile>\<^sub>M \<phi> \<and> M \<Turnstile>\<^sub>M \<^bold>\<not> \<Phi> \<longrightarrow> M \<Turnstile>\<^sub>M \<psi>)\<close> by simp
-            moreover have \<open>n = fst s\<close> using f1 by simp
-            then have \<open>?\<T> n = ?\<T>' n\<close> using \<open>?\<T> (fst s) = ?\<T>' (fst s)\<close> by blast
-            moreover have \<open>\<M>* ?\<T> (basic n) M = \<M>* ?\<T>' (basic n) M\<close> 
-            proof (cases M)
-              case (Pair \<Sigma> \<Gamma>)
-              then have \<open>\<M>* ?\<T> (basic n) M = \<M>* ?\<T> (basic n) (\<Sigma>, \<Gamma>)\<close> by simp
-              also have \<open>\<M>* ?\<T> (basic n) (\<Sigma>, \<Gamma>) = (case ?\<T> n (\<Sigma>, \<Gamma>) of Some \<Sigma>' \<Rightarrow> Some (\<Sigma>', \<Gamma> - {\<psi> \<in> \<Gamma>. \<Sigma>' \<Turnstile>\<^sub>L \<psi>}) | _ \<Rightarrow> None)\<close> by simp
-              also have \<open>\<dots> = (case ?\<T>' n (\<Sigma>, \<Gamma>) of Some \<Sigma>' \<Rightarrow> Some (\<Sigma>', \<Gamma> - {\<psi> \<in> \<Gamma>. \<Sigma>' \<Turnstile>\<^sub>L \<psi>}) | _ \<Rightarrow> None)\<close> using \<open>?\<T> n = ?\<T>' n\<close> by simp
-              also have \<open>\<dots> = \<M>* ?\<T>' (basic n) (\<Sigma>, \<Gamma>)\<close> by simp
-              finally show \<open>\<M>* ?\<T> (basic n) M = \<M>* ?\<T>' (basic n) M\<close> using Pair by simp
+          fix ht
+          assume \<open>ht \<in> set hts\<close>
+          show \<open>\<forall>M. complies_ht M ?\<T> \<Phi> (the (htb_basic_unpack ht))\<close>
+          proof
+            fix M
+            show \<open>complies_ht M ?\<T> \<Phi> (the (htb_basic_unpack ht))\<close>
+            proof (cases \<open>(the (htb_basic_unpack ht))\<close>)
+              case (fields \<phi> n' \<psi>)
+              have \<open>s\<in>set S \<and> fst s = fst s\<close> using \<open>s \<in> set S\<close> by simp
+              moreover have \<open>\<forall>s'. s'\<in>set S \<and> fst s = fst s' \<longrightarrow> s' = s\<close> using \<open>distinct (map fst S)\<close>
+                by (metis member eq_key_imp_eq_value prod.collapse)
+              ultimately have \<open>(THE s'. s'\<in>set S \<and> fst s = fst s') = s\<close> using the_equality by auto
+              then have \<open>?\<T> (fst s) = (SOME \<T>. complies_hts s \<T>) (fst s)\<close> (is \<open>?\<T> (fst s) = ?\<T>' (fst s)\<close>) using member by simp
+              have \<open>\<exists>\<T>. complies_hts s \<T>\<close> using assms(2) member by simp
+              then have \<open>complies_hts s ?\<T>'\<close> using someI_ex[where ?P=\<open>complies_hts s\<close>] by simp
+              then have \<open>\<forall>ht\<in>set hts. is_htb_basic ht \<and> (\<forall>M. complies_ht M ?\<T>' \<Phi> (the (htb_basic_unpack ht)))\<close> 
+                using f1 complies_hts_def by fastforce
+              with f1 \<open>ht \<in> set hts\<close> have \<open>\<forall>M. complies_ht M ?\<T>' \<Phi> (the (htb_basic_unpack ht))\<close> by simp
+              then have \<open>complies_ht M ?\<T>' \<Phi> (the (htb_basic_unpack ht))\<close> by blast
+              moreover have \<open>n = n'\<close> 
+                using fields assms(1) f1 member \<open>ht \<in> set hts\<close> unfolding is_ht_specification_def by fastforce
+              ultimately have \<open>complies_ht M ?\<T>' \<Phi> (\<phi>, n, \<psi>)\<close> using fields by simp
+              then have 
+                \<open>(M \<Turnstile>\<^sub>M \<Phi> \<longleftrightarrow> ?\<T>' n M \<noteq> None) \<and>
+                (\<not> (fst M) \<^bold>\<Turnstile>\<^sub>P \<^bold>\<bottom> \<longrightarrow> ?\<T>' n M \<noteq> None \<longrightarrow> \<not>the (?\<T>' n M) \<^bold>\<Turnstile>\<^sub>P \<^bold>\<bottom>) \<and>
+                (M \<Turnstile>\<^sub>M \<phi> \<and> M \<Turnstile>\<^sub>M \<Phi> \<longrightarrow> the (\<M>* ?\<T>' (basic n) M) \<Turnstile>\<^sub>M \<psi>) \<and>
+                (M \<Turnstile>\<^sub>M \<phi> \<and> M \<Turnstile>\<^sub>M \<^bold>\<not> \<Phi> \<longrightarrow> M \<Turnstile>\<^sub>M \<psi>)\<close> by simp
+              moreover have \<open>n = fst s\<close> using f1 by simp
+              then have \<open>?\<T> n = ?\<T>' n\<close> using \<open>?\<T> (fst s) = ?\<T>' (fst s)\<close> by blast
+              moreover have \<open>\<M>* ?\<T> (basic n) M = \<M>* ?\<T>' (basic n) M\<close> 
+              proof (cases M)
+                case (Pair \<Sigma> \<Gamma>)
+                then have \<open>\<M>* ?\<T> (basic n) M = \<M>* ?\<T> (basic n) (\<Sigma>, \<Gamma>)\<close> by simp
+                also have \<open>\<M>* ?\<T> (basic n) (\<Sigma>, \<Gamma>) = (case ?\<T> n (\<Sigma>, \<Gamma>) of Some \<Sigma>' \<Rightarrow> Some (\<Sigma>', \<Gamma> - {\<psi> \<in> \<Gamma>. \<Sigma>' \<^bold>\<Turnstile>\<^sub>P \<psi>}) | _ \<Rightarrow> None)\<close> by simp
+                also have \<open>\<dots> = (case ?\<T>' n (\<Sigma>, \<Gamma>) of Some \<Sigma>' \<Rightarrow> Some (\<Sigma>', \<Gamma> - {\<psi> \<in> \<Gamma>. \<Sigma>' \<^bold>\<Turnstile>\<^sub>P \<psi>}) | _ \<Rightarrow> None)\<close> using \<open>?\<T> n = ?\<T>' n\<close> by simp
+                also have \<open>\<dots> = \<M>* ?\<T>' (basic n) (\<Sigma>, \<Gamma>)\<close> by simp
+                finally show \<open>\<M>* ?\<T> (basic n) M = \<M>* ?\<T>' (basic n) M\<close> using Pair by simp
+              qed
+              ultimately have 
+                \<open>(M \<Turnstile>\<^sub>M \<Phi> \<longleftrightarrow> ?\<T> n M \<noteq> None) \<and>
+                (\<not> (fst M) \<^bold>\<Turnstile>\<^sub>P \<^bold>\<bottom> \<longrightarrow> ?\<T> n M \<noteq> None \<longrightarrow> \<not>the (?\<T> n M) \<^bold>\<Turnstile>\<^sub>P \<^bold>\<bottom>) \<and>
+                (M \<Turnstile>\<^sub>M \<phi> \<and> M \<Turnstile>\<^sub>M \<Phi> \<longrightarrow> the (\<M>* ?\<T> (basic n) M) \<Turnstile>\<^sub>M \<psi>) \<and>
+                (M \<Turnstile>\<^sub>M \<phi> \<and> M \<Turnstile>\<^sub>M \<^bold>\<not> \<Phi> \<longrightarrow> M \<Turnstile>\<^sub>M \<psi>)\<close> by simp
+              then have \<open>complies_ht M ?\<T> \<Phi> (\<phi>, n, \<psi>)\<close> by simp
+              with \<open>n = n'\<close> show ?thesis using fields by simp
             qed
-            ultimately have 
-              \<open>(M \<Turnstile>\<^sub>M \<Phi> \<longleftrightarrow> ?\<T> n M \<noteq> None) \<and>
-              (\<not> (fst M) \<Turnstile>\<^sub>L \<bottom>\<^sub>L \<longrightarrow> ?\<T> n M \<noteq> None \<longrightarrow> \<not>the (?\<T> n M) \<Turnstile>\<^sub>L \<bottom>\<^sub>L) \<and>
-              (M \<Turnstile>\<^sub>M \<phi> \<and> M \<Turnstile>\<^sub>M \<Phi> \<longrightarrow> the (\<M>* ?\<T> (basic n) M) \<Turnstile>\<^sub>M \<psi>) \<and>
-              (M \<Turnstile>\<^sub>M \<phi> \<and> M \<Turnstile>\<^sub>M \<^bold>\<not> \<Phi> \<longrightarrow> M \<Turnstile>\<^sub>M \<psi>)\<close> by simp
-            then have \<open>complies_ht M ?\<T> \<Phi> (\<phi>, n, \<psi>)\<close> by simp
-            with \<open>n = n'\<close> show ?thesis using fields by simp
           qed
         qed
+        moreover have \<open>\<forall>ht\<in>set hts. is_htb_basic ht\<close> 
+          using assms(1) f1 \<open>s \<in> set S\<close> unfolding is_ht_specification_def by simp
+        ultimately show ?thesis using f1 complies_hts_def by simp
       qed
-      moreover have \<open>\<forall>ht\<in>set hts. is_htb_basic ht\<close> 
-        using assms(1) f1 \<open>s \<in> set S\<close> unfolding is_ht_specification_def by simp
-      ultimately show ?thesis using f1 complies_hts_def by simp
     qed
-    then show \<open>complies_hts s ?\<T> \<and> (\<forall>n. n \<notin> set (map fst S) \<longrightarrow> (\<forall>M. ?\<T> n M = None))\<close> by simp
+  next
+    show \<open>\<forall>n. n \<notin> set (map fst S) \<longrightarrow> (\<forall>M. ?\<T> n M = None)\<close> by simp
   qed
 qed
-
-\<comment> \<open>Definition used in proofs to put less strain on Isabelle's simplification methods.\<close>
-definition next_state_reqs where
-\<open>next_state_reqs M hts M' \<equiv> 
-  (\<not> fst M \<Turnstile>\<^sub>L \<bottom>\<^sub>L \<longrightarrow> \<not> fst M' \<Turnstile>\<^sub>L \<bottom>\<^sub>L) \<and> 
-  (snd M' = snd M - {\<psi> \<in> snd M. fst M' \<Turnstile>\<^sub>L \<psi>}) \<and> 
-  (\<forall>ht \<in> { ht \<in> set hts. M \<Turnstile>\<^sub>M pre ht }. M' \<Turnstile>\<^sub>M post ht)\<close>
 
 \<comment> \<open>If S is a valid specification, there exists a belief update function (model) that S complies to.\<close>
 lemma model_exists: \<open>is_ht_specification S \<Longrightarrow> \<exists>\<T>. complies S \<T>\<close>
@@ -175,7 +173,7 @@ proof -
       case f1: (fields n \<Phi> hts)
       have \<open>\<exists>\<T>. complies_hts (n, \<Phi>, hts) \<T>\<close> 
       proof
-        let ?\<T> = \<open>\<lambda>n M. if M \<Turnstile>\<^sub>M \<Phi> then Some (fst (SOME M'. next_state_reqs M hts M')) else None\<close>
+        let ?\<T> = \<open>\<lambda>n M. if M \<Turnstile>\<^sub>M \<Phi> then Some (SOME \<Sigma>. satisfiable_base M hts \<Sigma>) else None\<close>
         have \<open>\<forall>ht\<in>set hts. is_htb_basic ht \<and> (\<forall>M. complies_ht M ?\<T> \<Phi> (the (htb_basic_unpack ht)))\<close>
         proof
           fix ht
@@ -193,70 +191,72 @@ proof -
                 moreover have \<open>complies_ht M ?\<T> \<Phi> (\<phi>, n, \<psi>)\<close>
                 proof (cases \<open>M \<Turnstile>\<^sub>M \<Phi>\<close>)
                   case True
-                  then have nM: \<open>?\<T> n M = Some (fst (SOME M'. next_state_reqs M hts M'))\<close> by simp
+                  then have nM: \<open>?\<T> n M = Some (SOME \<Sigma>. satisfiable_base M hts \<Sigma>)\<close> by simp
                   moreover from sat have 
-                    \<open>let (_, \<Phi>, hts) = s; sat_hts = { ht \<in> set hts. M \<Turnstile>\<^sub>M pre ht } in
-                      (M \<Turnstile>\<^sub>M \<Phi> \<longrightarrow> (\<exists>M'. (\<not> fst M \<Turnstile>\<^sub>L \<bottom>\<^sub>L \<longrightarrow> \<not> fst M' \<Turnstile>\<^sub>L \<bottom>\<^sub>L) \<and> 
-                        (snd M' = snd M - {\<psi> \<in> snd M. fst M' \<Turnstile>\<^sub>L \<psi>}) \<and> 
-                        (\<forall>ht \<in> sat_hts. M' \<Turnstile>\<^sub>M post ht))) \<and>
-                      (M \<Turnstile>\<^sub>M \<^bold>\<not> \<Phi> \<longrightarrow> (\<forall>ht \<in> sat_hts. M \<Turnstile>\<^sub>M post ht))\<close> 
-                    using \<open>s \<in> set S\<close> unfolding satisfiable_def by blast
+                    \<open>\<forall>s \<in> set S. 
+                        ((M \<Turnstile>\<^sub>M (fst (snd s)) \<longrightarrow> 
+                          (\<exists> \<Sigma>. 
+                            (\<not> fst M \<^bold>\<Turnstile>\<^sub>P \<^bold>\<bottom> \<longrightarrow> \<not> \<Sigma> \<^bold>\<Turnstile>\<^sub>P \<^bold>\<bottom>) \<and> 
+                            (\<forall>ht \<in> set (snd (snd s)). M \<Turnstile>\<^sub>M pre ht \<longrightarrow> (\<Sigma>, snd M - {\<psi> \<in> snd M. \<Sigma> \<^bold>\<Turnstile>\<^sub>P \<psi>}) \<Turnstile>\<^sub>M post ht))) \<and>
+                            (M \<Turnstile>\<^sub>M \<^bold>\<not> (fst (snd s)) \<longrightarrow> (\<forall>ht \<in> set (snd (snd s)). M \<Turnstile>\<^sub>M pre ht \<longrightarrow> M \<Turnstile>\<^sub>M post ht)))\<close>
+                    unfolding satisfiable_def satisfiable_elem_def satisfiable_base_def by blast
+                  with \<open>s \<in> set S\<close> have 
+                    \<open>((M \<Turnstile>\<^sub>M (fst (snd s)) \<longrightarrow> 
+                        (\<exists> \<Sigma>. 
+                          (\<not> fst M \<^bold>\<Turnstile>\<^sub>P \<^bold>\<bottom> \<longrightarrow> \<not> \<Sigma> \<^bold>\<Turnstile>\<^sub>P \<^bold>\<bottom>) \<and> 
+                          (\<forall>ht \<in> set (snd (snd s)). M \<Turnstile>\<^sub>M pre ht \<longrightarrow> (\<Sigma>, snd M - {\<psi> \<in> snd M. \<Sigma> \<^bold>\<Turnstile>\<^sub>P \<psi>}) \<Turnstile>\<^sub>M post ht))) \<and>
+                          (M \<Turnstile>\<^sub>M \<^bold>\<not> (fst (snd s)) \<longrightarrow> (\<forall>ht \<in> set (snd (snd s)). M \<Turnstile>\<^sub>M pre ht \<longrightarrow> M \<Turnstile>\<^sub>M post ht)))\<close>
+                    by simp
                   with f1 True have ex:
-                    \<open>\<exists>M'. next_state_reqs M hts M'\<close>
-                    unfolding next_state_reqs_def by simp
-                  have \<open>\<forall>M'. next_state_reqs M hts M' \<longrightarrow> \<not> (fst M) \<Turnstile>\<^sub>L \<bottom>\<^sub>L \<longrightarrow> ?\<T> n M \<noteq> None \<longrightarrow> \<not> fst M' \<Turnstile>\<^sub>L \<bottom>\<^sub>L\<close>
+                    \<open>\<exists>\<Sigma>. satisfiable_base M hts \<Sigma>\<close>
+                    unfolding satisfiable_base_def by simp
+                  have \<open>\<forall>\<Sigma>. satisfiable_base M hts \<Sigma> \<longrightarrow> \<not> (fst M) \<^bold>\<Turnstile>\<^sub>P \<^bold>\<bottom> \<longrightarrow> ?\<T> n M \<noteq> None \<longrightarrow> \<not> \<Sigma> \<^bold>\<Turnstile>\<^sub>P \<^bold>\<bottom>\<close>
                   proof
-                    fix M'
-                    show \<open>next_state_reqs M hts M' \<longrightarrow> \<not> (fst M) \<Turnstile>\<^sub>L \<bottom>\<^sub>L \<longrightarrow> ?\<T> n M \<noteq> None \<longrightarrow> \<not> fst M' \<Turnstile>\<^sub>L \<bottom>\<^sub>L\<close> 
+                    fix \<Sigma>
+                    show \<open>satisfiable_base M hts \<Sigma> \<longrightarrow> \<not> (fst M) \<^bold>\<Turnstile>\<^sub>P \<^bold>\<bottom> \<longrightarrow> ?\<T> n M \<noteq> None \<longrightarrow> \<not> \<Sigma> \<^bold>\<Turnstile>\<^sub>P \<^bold>\<bottom>\<close> 
                     proof
-                      assume \<open>next_state_reqs M hts M'\<close>
-                      then show \<open>\<not> (fst M) \<Turnstile>\<^sub>L \<bottom>\<^sub>L \<longrightarrow> ?\<T> n M \<noteq> None \<longrightarrow> \<not> fst M' \<Turnstile>\<^sub>L \<bottom>\<^sub>L\<close> 
-                        unfolding next_state_reqs_def by simp
+                      assume \<open>satisfiable_base M hts \<Sigma>\<close>
+                      then show \<open>\<not> (fst M) \<^bold>\<Turnstile>\<^sub>P \<^bold>\<bottom> \<longrightarrow> ?\<T> n M \<noteq> None \<longrightarrow> \<not> \<Sigma> \<^bold>\<Turnstile>\<^sub>P \<^bold>\<bottom>\<close> 
+                        unfolding satisfiable_base_def by simp
                     qed
                   qed
-                  with ex have \<open>\<not> (fst M) \<Turnstile>\<^sub>L \<bottom>\<^sub>L \<longrightarrow> ?\<T> n M \<noteq> None \<longrightarrow> \<not> fst (SOME M'. next_state_reqs M hts M') \<Turnstile>\<^sub>L \<bottom>\<^sub>L\<close>  
-                    using someI2[where ?P=\<open>next_state_reqs M hts\<close>] by blast
-                  moreover have \<open>\<forall>M'. next_state_reqs M hts M' \<longrightarrow> (M \<Turnstile>\<^sub>M \<phi> \<and> M \<Turnstile>\<^sub>M \<Phi> \<longrightarrow> M' \<Turnstile>\<^sub>M \<psi>)\<close>
+                  with ex have \<open>\<not> (fst M) \<^bold>\<Turnstile>\<^sub>P \<^bold>\<bottom> \<longrightarrow> ?\<T> n M \<noteq> None \<longrightarrow> \<not> (SOME \<Sigma>. satisfiable_base M hts \<Sigma>) \<^bold>\<Turnstile>\<^sub>P \<^bold>\<bottom>\<close>  
+                    using someI2[where ?P=\<open>satisfiable_base M hts\<close>] by blast
+                  moreover have \<open>\<forall>\<Sigma>. satisfiable_base M hts \<Sigma> \<longrightarrow> (M \<Turnstile>\<^sub>M \<phi> \<and> M \<Turnstile>\<^sub>M \<Phi> \<longrightarrow> (\<Sigma>, snd M - {\<psi> \<in> snd M. \<Sigma> \<^bold>\<Turnstile>\<^sub>P \<psi>}) \<Turnstile>\<^sub>M \<psi>)\<close>
                   proof
-                    fix M'
-                    show \<open>next_state_reqs M hts M' \<longrightarrow> (M \<Turnstile>\<^sub>M \<phi> \<and> M \<Turnstile>\<^sub>M \<Phi> \<longrightarrow> M' \<Turnstile>\<^sub>M \<psi>)\<close> 
+                    fix \<Sigma>
+                    show \<open>satisfiable_base M hts \<Sigma> \<longrightarrow> (M \<Turnstile>\<^sub>M \<phi> \<and> M \<Turnstile>\<^sub>M \<Phi> \<longrightarrow> (\<Sigma>, snd M - {\<psi> \<in> snd M. \<Sigma> \<^bold>\<Turnstile>\<^sub>P \<psi>}) \<Turnstile>\<^sub>M \<psi>)\<close> 
                     proof
-                      assume \<open>next_state_reqs M hts M'\<close>
-                      with \<open>ht \<in> set hts\<close> have \<open>M \<Turnstile>\<^sub>M pre ht \<longrightarrow> M' \<Turnstile>\<^sub>M post ht\<close> unfolding next_state_reqs_def by simp
+                      assume \<open>satisfiable_base M hts \<Sigma>\<close>
+                      with \<open>ht \<in> set hts\<close> have \<open>M \<Turnstile>\<^sub>M pre ht \<longrightarrow> (\<Sigma>, snd M - {\<psi> \<in> snd M. \<Sigma> \<^bold>\<Turnstile>\<^sub>P \<psi>}) \<Turnstile>\<^sub>M post ht\<close> unfolding satisfiable_base_def by simp
                       moreover from \<open>is_htb_basic ht\<close> have \<open>pre ht = \<phi>\<close> 
                         using fields unpack_sel(1) by fastforce
                       moreover from \<open>is_htb_basic ht\<close> have \<open>post ht = \<psi>\<close> 
                         using fields unpack_sel(2) by fastforce
-                      ultimately have \<open>M \<Turnstile>\<^sub>M \<phi> \<longrightarrow> M' \<Turnstile>\<^sub>M \<psi>\<close> by simp
-                      then show \<open>M \<Turnstile>\<^sub>M \<phi> \<and> M \<Turnstile>\<^sub>M \<Phi> \<longrightarrow> M' \<Turnstile>\<^sub>M \<psi>\<close> by simp
+                      ultimately have \<open>M \<Turnstile>\<^sub>M \<phi> \<longrightarrow> (\<Sigma>, snd M - {\<psi> \<in> snd M. \<Sigma> \<^bold>\<Turnstile>\<^sub>P \<psi>}) \<Turnstile>\<^sub>M \<psi>\<close> by simp
+                      then show \<open>M \<Turnstile>\<^sub>M \<phi> \<and> M \<Turnstile>\<^sub>M \<Phi> \<longrightarrow> (\<Sigma>, snd M - {\<psi> \<in> snd M. \<Sigma> \<^bold>\<Turnstile>\<^sub>P \<psi>}) \<Turnstile>\<^sub>M \<psi>\<close> by simp
                     qed
                   qed
-                  with ex have \<open>(M \<Turnstile>\<^sub>M \<phi> \<and> M \<Turnstile>\<^sub>M \<Phi> \<longrightarrow> (SOME M'. next_state_reqs M hts M') \<Turnstile>\<^sub>M \<psi>)\<close>
-                    using someI2[where ?P=\<open>next_state_reqs M hts\<close>] by blast
+                  with ex have \<open>(M \<Turnstile>\<^sub>M \<phi> \<and> M \<Turnstile>\<^sub>M \<Phi> \<longrightarrow> ((SOME \<Sigma>. satisfiable_base M hts \<Sigma>), snd M - {\<psi> \<in> snd M. (SOME \<Sigma>. satisfiable_base M hts \<Sigma>) \<^bold>\<Turnstile>\<^sub>P \<psi>}) \<Turnstile>\<^sub>M \<psi>)\<close>
+                    using someI2[where ?P=\<open>satisfiable_base M hts\<close>] by blast
                   ultimately have 
-                    \<open>(M \<Turnstile>\<^sub>M \<Phi> \<longleftrightarrow> Some (fst (SOME M'. next_state_reqs M hts M')) \<noteq> None) \<and>
-                      (\<not> (fst M) \<Turnstile>\<^sub>L \<bottom>\<^sub>L \<longrightarrow> \<not> fst (SOME M'. next_state_reqs M hts M') \<Turnstile>\<^sub>L \<bottom>\<^sub>L) \<and>
-                      (M \<Turnstile>\<^sub>M \<phi> \<and> M \<Turnstile>\<^sub>M \<Phi> \<longrightarrow> (SOME M'. next_state_reqs M hts M') \<Turnstile>\<^sub>M \<psi>) \<and> 
+                    \<open>(M \<Turnstile>\<^sub>M \<Phi> \<longleftrightarrow> Some (SOME \<Sigma>. satisfiable_base M hts \<Sigma>) \<noteq> None) \<and>
+                      (\<not> (fst M) \<^bold>\<Turnstile>\<^sub>P \<^bold>\<bottom> \<longrightarrow> \<not> (SOME \<Sigma>. satisfiable_base M hts \<Sigma>) \<^bold>\<Turnstile>\<^sub>P \<^bold>\<bottom>) \<and>
+                      (M \<Turnstile>\<^sub>M \<phi> \<and> M \<Turnstile>\<^sub>M \<Phi> \<longrightarrow> ((SOME \<Sigma>. satisfiable_base M hts \<Sigma>), snd M - {\<psi> \<in> snd M. (SOME \<Sigma>. satisfiable_base M hts \<Sigma>) \<^bold>\<Turnstile>\<^sub>P \<psi>}) \<Turnstile>\<^sub>M \<psi>) \<and> 
                       (M \<Turnstile>\<^sub>M \<phi> \<and> M \<Turnstile>\<^sub>M \<^bold>\<not> \<Phi> \<longrightarrow> M \<Turnstile>\<^sub>M \<psi>)\<close> 
                     using True by auto
-                  moreover have \<open>(SOME M'. next_state_reqs M hts M') \<Turnstile>\<^sub>M \<psi> \<longrightarrow> the (\<M>* ?\<T> (basic n) M) \<Turnstile>\<^sub>M \<psi>\<close> 
+                  moreover have \<open>((SOME \<Sigma>. satisfiable_base M hts \<Sigma>), snd M - {\<psi> \<in> snd M. (SOME \<Sigma>. satisfiable_base M hts \<Sigma>) \<^bold>\<Turnstile>\<^sub>P \<psi>}) \<Turnstile>\<^sub>M \<psi> \<longrightarrow> the (\<M>* ?\<T> (basic n) M) \<Turnstile>\<^sub>M \<psi>\<close> 
                   proof (cases M)
                     case (Pair \<Sigma> \<Gamma>)
                     show ?thesis 
                     proof
-                      assume entails: \<open>(SOME M'. next_state_reqs M hts M') \<Turnstile>\<^sub>M \<psi>\<close>
-                      from Pair have \<open>\<forall>M'. next_state_reqs M hts M' \<longrightarrow> snd M' = (snd M - {\<psi> \<in> snd M. fst M' \<Turnstile>\<^sub>L \<psi>})\<close> 
-                        unfolding next_state_reqs_def by simp
-                      with ex have \<open>snd (SOME M'. next_state_reqs M hts M') = snd M - {\<psi> \<in> snd M. fst (SOME M'. next_state_reqs M hts M') \<Turnstile>\<^sub>L \<psi>}\<close>  
-                        using someI2[where ?P=\<open>next_state_reqs M hts\<close>] by blast
-                      with entails have \<open>(fst (SOME M'. next_state_reqs M hts M'), snd M - {\<psi> \<in> snd M. fst (SOME M'. next_state_reqs M hts M') \<Turnstile>\<^sub>L \<psi>}) \<Turnstile>\<^sub>M \<psi>\<close>
-                        by (metis prod.collapse)
+                      assume entails: \<open>((SOME \<Sigma>. satisfiable_base M hts \<Sigma>), snd M - {\<psi> \<in> snd M. (SOME \<Sigma>. satisfiable_base M hts \<Sigma>) \<^bold>\<Turnstile>\<^sub>P \<psi>}) \<Turnstile>\<^sub>M \<psi>\<close>
                       with nM Pair show \<open>the (\<M>* ?\<T> (basic n) M) \<Turnstile>\<^sub>M \<psi>\<close> by auto
                     qed
                   qed
                   ultimately have 
                     \<open>(M \<Turnstile>\<^sub>M \<Phi> \<longleftrightarrow> ?\<T> n M \<noteq> None) \<and>
-                      (\<not> (fst M) \<Turnstile>\<^sub>L \<bottom>\<^sub>L \<longrightarrow> ?\<T> n M \<noteq> None \<longrightarrow> \<not> the (?\<T> n M) \<Turnstile>\<^sub>L \<bottom>\<^sub>L) \<and>
+                      (\<not> (fst M) \<^bold>\<Turnstile>\<^sub>P \<^bold>\<bottom> \<longrightarrow> ?\<T> n M \<noteq> None \<longrightarrow> \<not> the (?\<T> n M) \<^bold>\<Turnstile>\<^sub>P \<^bold>\<bottom>) \<and>
                       (M \<Turnstile>\<^sub>M \<phi> \<and> M \<Turnstile>\<^sub>M \<Phi> \<longrightarrow> the (\<M>* ?\<T> (basic n) M) \<Turnstile>\<^sub>M \<psi>) \<and> 
                       (M \<Turnstile>\<^sub>M \<phi> \<and> M \<Turnstile>\<^sub>M \<^bold>\<not> \<Phi> \<longrightarrow> M \<Turnstile>\<^sub>M \<psi>)\<close> 
                     using nM by simp
@@ -267,14 +267,18 @@ proof -
                   then have \<open>M \<Turnstile>\<^sub>M \<phi> \<and> M \<Turnstile>\<^sub>M \<^bold>\<not> \<Phi> \<longrightarrow> M \<Turnstile>\<^sub>M \<psi>\<close> 
                   proof -
                     from sat have 
-                      \<open>let (_, \<Phi>, hts) = s; sat_hts = { ht \<in> set hts. M \<Turnstile>\<^sub>M pre ht } in
-                        (M \<Turnstile>\<^sub>M \<Phi> \<longrightarrow> (\<exists>M'. (\<not> fst M \<Turnstile>\<^sub>L \<bottom>\<^sub>L \<longrightarrow> \<not> fst M' \<Turnstile>\<^sub>L \<bottom>\<^sub>L) \<and> 
-                          (snd M' = snd M - {\<psi> \<in> snd M. fst M' \<Turnstile>\<^sub>L \<psi>}) \<and> 
-                          (\<forall>ht \<in> sat_hts. M' \<Turnstile>\<^sub>M post ht))) \<and>
-                        (M \<Turnstile>\<^sub>M \<^bold>\<not> \<Phi> \<longrightarrow> (\<forall>ht \<in> sat_hts. M \<Turnstile>\<^sub>M post ht))\<close> 
-                      using \<open>s \<in> set S\<close> unfolding satisfiable_def by blast
-                    then have \<open>\<forall>ht \<in> { ht \<in> set hts. M \<Turnstile>\<^sub>M pre ht }. M \<Turnstile>\<^sub>M post ht\<close> 
-                      using False f1 by simp
+                      \<open>\<forall>s \<in> set S.                         
+                        ((M \<Turnstile>\<^sub>M (fst (snd s)) \<longrightarrow> 
+                          (\<exists> \<Sigma>. 
+                            (\<not> fst M \<^bold>\<Turnstile>\<^sub>P \<^bold>\<bottom> \<longrightarrow> \<not> \<Sigma> \<^bold>\<Turnstile>\<^sub>P \<^bold>\<bottom>) \<and> 
+                            (\<forall>ht \<in> set (snd (snd s)). M \<Turnstile>\<^sub>M pre ht \<longrightarrow> (\<Sigma>, snd M - {\<psi> \<in> snd M. \<Sigma> \<^bold>\<Turnstile>\<^sub>P \<psi>}) \<Turnstile>\<^sub>M post ht))) \<and>
+                            (M \<Turnstile>\<^sub>M \<^bold>\<not> (fst (snd s)) \<longrightarrow> (\<forall>ht \<in> set (snd (snd s)). M \<Turnstile>\<^sub>M pre ht \<longrightarrow> M \<Turnstile>\<^sub>M post ht)))\<close>
+                      using \<open>s \<in> set S\<close> f1 
+                      unfolding satisfiable_def satisfiable_elem_def satisfiable_base_def 
+                      by blast
+                    with \<open>s \<in> set S\<close> False have 
+                      \<open>\<forall>ht \<in> set hts. M \<Turnstile>\<^sub>M pre ht \<longrightarrow> M \<Turnstile>\<^sub>M post ht\<close> 
+                      using \<open>s \<in> set S\<close> f1 unfolding satisfiable_def by auto
                     with \<open>ht \<in> set hts\<close> have \<open>M \<Turnstile>\<^sub>M pre ht \<longrightarrow> M \<Turnstile>\<^sub>M post ht\<close> by simp
                     moreover from \<open>is_htb_basic ht\<close> have \<open>pre ht = \<phi>\<close> 
                       using fields unpack_sel(1) by fastforce
@@ -307,7 +311,6 @@ locale single_agent_program = single_agent +
   fixes
     Sp :: ht_specification
   assumes
-    Sp_valid: \<open>is_ht_specification Sp\<close> and 
     \<T>_complies: \<open>complies Sp \<T>\<close>
 
 context single_agent_program begin
@@ -321,7 +324,7 @@ inductive derive\<^sub>H :: \<open>hoare_triple \<Rightarrow> bool\<close> (\<op
   import: \<open>(n, \<Phi>, hts) \<in> set Sp \<Longrightarrow> \<^bold>{ \<phi> \<^bold>} (basic n) \<^bold>{ \<psi> \<^bold>} \<in> set hts \<Longrightarrow> \<turnstile>\<^sub>H \<^bold>{ \<phi> \<^bold>} (basic n) \<^bold>{ \<psi> \<^bold>}\<close> |
   \<comment> \<open>Persistence of goals\<close>
   (*persist: \<open>\<not> is_drop a \<Longrightarrow> \<turnstile>\<^sub>H \<^bold>{ G \<Phi> \<^bold>} a \<^bold>{ (B \<Phi>) \<^bold>\<or> (G \<Phi>) \<^bold>}\<close> |*)
-  persist: \<open>\<not> is_drop a \<Longrightarrow> \<turnstile>\<^sub>H \<^bold>{ (G \<Phi>)  \<^bold>} a \<^bold>{ (B \<Phi>) \<^bold>\<or> (G \<Phi>) \<^bold>}\<close> |
+  persist: \<open>\<not> is_drop a \<Longrightarrow> \<turnstile>\<^sub>H \<^bold>{ (G \<Phi>) \<^bold>} a \<^bold>{ (B \<Phi>) \<^bold>\<or> (G \<Phi>) \<^bold>}\<close> |
   \<comment> \<open>Infeasible actions\<close>
   inf:  \<open>\<turnstile>\<^sub>E ((\<phi>\<^sup>E) \<^bold>\<longrightarrow> \<^bold>\<not>(enabledb a)) \<Longrightarrow> \<turnstile>\<^sub>H \<^bold>{ \<phi> \<^bold>} a \<^bold>{ \<phi> \<^bold>}\<close> |
   \<comment> \<open>Frame properties on beliefs for adopt and drop\<close>
@@ -330,12 +333,12 @@ inductive derive\<^sub>H :: \<open>hoare_triple \<Rightarrow> bool\<close> (\<op
   dropB: \<open>\<turnstile>\<^sub>H \<^bold>{ B \<Phi> \<^bold>} (drop \<psi>) \<^bold>{ B \<Phi> \<^bold>}\<close> |
   dropNegB: \<open>\<turnstile>\<^sub>H \<^bold>{ \<^bold>\<not> (B \<Phi>) \<^bold>} (drop \<psi>) \<^bold>{ \<^bold>\<not> (B \<Phi>) \<^bold>}\<close> |
   \<comment> \<open>Effects of adopt\<close>
-  adoptBG: \<open>\<not> {} \<Turnstile>\<^sub>P (\<^bold>\<not> \<Phi>) \<Longrightarrow> \<turnstile>\<^sub>H \<^bold>{ \<^bold>\<not> (B \<Phi>) \<^bold>} (adopt \<Phi>) \<^bold>{ G \<Phi> \<^bold>}\<close> |
+  adoptBG: \<open>\<not> \<Turnstile>\<^sub>P (\<^bold>\<not> \<Phi>) \<Longrightarrow> \<turnstile>\<^sub>H \<^bold>{ \<^bold>\<not> (B \<Phi>) \<^bold>} (adopt \<Phi>) \<^bold>{ G \<Phi> \<^bold>}\<close> |
   \<comment> \<open>Non-effect of adopt\<close>
   adoptG: \<open>\<turnstile>\<^sub>H \<^bold>{ G \<Phi> \<^bold>} (adopt \<psi>) \<^bold>{ G \<Phi> \<^bold>}\<close> |
-  adoptNegG: \<open>\<not> {} \<Turnstile>\<^sub>P \<psi> \<^bold>\<longrightarrow> \<Phi> \<Longrightarrow> \<turnstile>\<^sub>H \<^bold>{ \<^bold>\<not> (G \<Phi>) \<^bold>} (adopt \<psi>) \<^bold>{ \<^bold>\<not> (G \<Phi>) \<^bold>}\<close> |
+  adoptNegG: \<open>\<not> \<Turnstile>\<^sub>P (\<psi> \<^bold>\<longrightarrow> \<Phi>) \<Longrightarrow> \<turnstile>\<^sub>H \<^bold>{ \<^bold>\<not> (G \<Phi>) \<^bold>} (adopt \<psi>) \<^bold>{ \<^bold>\<not> (G \<Phi>) \<^bold>}\<close> |
   \<comment> \<open>Effects of drop\<close>
-  dropG: \<open>{} \<Turnstile>\<^sub>P \<Phi> \<^bold>\<longrightarrow> \<psi> \<Longrightarrow> \<turnstile>\<^sub>H \<^bold>{ G \<Phi> \<^bold>} (drop \<psi>) \<^bold>{ \<^bold>\<not> (G \<Phi>) \<^bold>}\<close> |
+  dropG: \<open>\<Turnstile>\<^sub>P (\<Phi> \<^bold>\<longrightarrow> \<psi>) \<Longrightarrow> \<turnstile>\<^sub>H \<^bold>{ G \<Phi> \<^bold>} (drop \<psi>) \<^bold>{ \<^bold>\<not> (G \<Phi>) \<^bold>}\<close> |
   \<comment> \<open>Non-effects of drop\<close>
   dropNegG: \<open>\<turnstile>\<^sub>H \<^bold>{ \<^bold>\<not>(G \<Phi>) \<^bold>} (drop \<psi>) \<^bold>{ \<^bold>\<not>(G \<Phi>) \<^bold>}\<close> |
   dropGCon: \<open>\<turnstile>\<^sub>H \<^bold>{ \<^bold>\<not>(G (\<Phi> \<^bold>\<and> \<psi>)) \<^bold>\<and> (G \<Phi>) \<^bold>} (drop \<psi>) \<^bold>{ G \<Phi> \<^bold>}\<close> |
@@ -423,11 +426,11 @@ next
             case (basic n)
             with notNone have \<open>\<M> (basic n) (\<Sigma>, \<Gamma>) \<noteq> None\<close> by simp
             then obtain \<Sigma>' where \<Sigma>': \<open>\<T> n (\<Sigma>, \<Gamma>) = Some \<Sigma>'\<close> by fastforce
-            then have mst_unfold: \<open>\<M> (basic n) (\<Sigma>, \<Gamma>) = Some (\<Sigma>', \<Gamma> - {\<psi> \<in> \<Gamma>. \<Sigma>' \<Turnstile>\<^sub>L \<psi>})\<close>
+            then have mst_unfold: \<open>\<M> (basic n) (\<Sigma>, \<Gamma>) = Some (\<Sigma>', \<Gamma> - {\<psi> \<in> \<Gamma>. \<Sigma>' \<^bold>\<Turnstile>\<^sub>P \<psi>})\<close>
                               (is \<open>\<M> (basic n) (\<Sigma>, \<Gamma>) = Some (\<Sigma>', ?\<Gamma>')\<close>) 
               by simp
             then show ?thesis 
-            proof (cases \<open>\<Sigma>' \<Turnstile>\<^sub>L \<Phi>\<close>)
+            proof (cases \<open>\<Sigma>' \<^bold>\<Turnstile>\<^sub>P \<Phi>\<close>)
               case True
               then have \<open>(\<Sigma>', ?\<Gamma>') \<Turnstile>\<^sub>M (B \<Phi>) \<^bold>\<or> (G \<Phi>)\<close> by auto
               with mst_unfold show ?thesis using basic Pair by simp
@@ -439,7 +442,7 @@ next
             qed
           next
             case (adopt \<Phi>')
-            have \<open>\<M> (adopt \<Phi>') (\<Sigma>, \<Gamma>) = (if \<not> {} \<Turnstile>\<^sub>L \<^bold>\<not> \<Phi>' \<and> \<not> \<Sigma> \<Turnstile>\<^sub>L \<Phi>' then Some (\<Sigma>, \<Gamma> \<union> {\<Phi>'}) else None)\<close> 
+            have \<open>\<M> (adopt \<Phi>') (\<Sigma>, \<Gamma>) = (if \<not> \<Turnstile>\<^sub>P (\<^bold>\<not> \<Phi>') \<and> \<not> \<Sigma> \<^bold>\<Turnstile>\<^sub>P \<Phi>' then Some (\<Sigma>, \<Gamma> \<union> {\<Phi>'}) else None)\<close> 
               by simp
             with notNone have \<open>\<M> (adopt \<Phi>') (\<Sigma>, \<Gamma>) = Some (\<Sigma>, \<Gamma> \<union> {\<Phi>'})\<close> using adopt by metis
             then show ?thesis using adopt Pair asm by simp
@@ -477,11 +480,11 @@ next
         proof
           from \<open>M \<Turnstile>\<^sub>E (?\<phi>\<^sup>E)\<close> show \<open>M \<Turnstile>\<^sub>E enabledb ?a\<close> using adoptBG by (cases M) simp
           with \<open>M \<Turnstile>\<^sub>E (?\<phi>\<^sup>E)\<close> adoptBG have s: \<open>\<M> ?a M = Some (fst M, snd M \<union> {\<Phi>})\<close> by (cases M) simp
-          then have \<open>\<exists>\<gamma>\<in>snd (the (\<M> ?a M)). {} \<Turnstile>\<^sub>L \<gamma> \<^bold>\<longrightarrow> \<Phi>\<close> by simp
+          then have \<open>\<exists>\<gamma>\<in>snd (the (\<M> ?a M)). \<Turnstile>\<^sub>P (\<gamma> \<^bold>\<longrightarrow> \<Phi>)\<close> by simp
           moreover {
             from s have \<open>fst (the (\<M> ?a M)) = fst M\<close> by simp
-            moreover have \<open>\<not> fst M \<Turnstile>\<^sub>L \<Phi>\<close> using \<open>M \<Turnstile>\<^sub>E (?\<phi>\<^sup>E)\<close> by (cases M) simp
-            ultimately have \<open>\<not> fst (the (\<M> ?a M)) \<Turnstile>\<^sub>L \<Phi>\<close> by simp
+            moreover have \<open>\<not> fst M \<^bold>\<Turnstile>\<^sub>P \<Phi>\<close> using \<open>M \<Turnstile>\<^sub>E (?\<phi>\<^sup>E)\<close> by (cases M) simp
+            ultimately have \<open>\<not> fst (the (\<M> ?a M)) \<^bold>\<Turnstile>\<^sub>P \<Phi>\<close> by simp
           }
           ultimately show \<open>the (\<M> ?a M) \<Turnstile>\<^sub>M ?\<psi>\<close> 
             using semantics\<^sub>M'.simps(2)[where \<Sigma>=\<open>fst (the (\<M> ?a M))\<close> and \<Gamma>=\<open>snd (the (\<M> ?a M))\<close>] 
@@ -509,16 +512,16 @@ next
       proof
         assume \<open>M \<Turnstile>\<^sub>M ?\<phi>\<close>      
         with dropGCon have pre:
-          \<open>\<not> fst M \<Turnstile>\<^sub>L \<Phi> \<and> 
-           \<not> (\<exists>\<gamma>\<in>snd M. {} \<Turnstile>\<^sub>L \<gamma> \<^bold>\<longrightarrow> (\<Phi> \<^bold>\<and> \<psi>)) \<and> 
-              (\<exists>\<gamma>\<in>snd M. {} \<Turnstile>\<^sub>L \<gamma> \<^bold>\<longrightarrow> \<Phi>)\<close>  
+          \<open>\<not> fst M \<^bold>\<Turnstile>\<^sub>P \<Phi> \<and> 
+           \<not> (\<exists>\<gamma>\<in>snd M. \<Turnstile>\<^sub>P (\<gamma> \<^bold>\<longrightarrow> (\<Phi> \<^bold>\<and> \<psi>))) \<and> 
+              (\<exists>\<gamma>\<in>snd M. \<Turnstile>\<^sub>P (\<gamma> \<^bold>\<longrightarrow> \<Phi>))\<close>  
           by (cases M) auto
-        moreover from pre obtain \<gamma> where gamma: \<open>\<gamma> \<in> snd M \<and> {} \<Turnstile>\<^sub>L \<gamma> \<^bold>\<longrightarrow> \<Phi>\<close> by auto
-        moreover have aM: \<open>\<M> ?a M = Some (fst M, snd M - {\<gamma> \<in> snd M. {\<gamma>} \<Turnstile>\<^sub>L \<psi>})\<close> (is \<open>\<dots> = Some ?M'\<close>) 
+        moreover from pre obtain \<gamma> where gamma: \<open>\<gamma> \<in> snd M \<and> \<Turnstile>\<^sub>P (\<gamma> \<^bold>\<longrightarrow> \<Phi>)\<close> by auto
+        moreover have aM: \<open>\<M> ?a M = Some (fst M, snd M - {\<gamma> \<in> snd M. {\<gamma>} \<^bold>\<Turnstile>\<^sub>P \<psi>})\<close> (is \<open>\<dots> = Some ?M'\<close>) 
           by (cases M) simp
-        ultimately have \<open>\<not> fst ?M' \<Turnstile>\<^sub>L \<Phi>\<close> by simp
-        moreover from pre gamma have \<open>\<not> {\<gamma>} \<Turnstile>\<^sub>L \<Phi> \<^bold>\<and> \<psi>\<close> by auto
-        with gamma have \<open>\<exists>\<gamma>\<in>snd ?M'. {} \<Turnstile>\<^sub>L \<gamma> \<^bold>\<longrightarrow> \<Phi>\<close> by auto
+        ultimately have \<open>\<not> fst ?M' \<^bold>\<Turnstile>\<^sub>P \<Phi>\<close> by simp
+        moreover from pre gamma have \<open>\<not> {\<gamma>} \<^bold>\<Turnstile>\<^sub>P (\<Phi> \<^bold>\<and> \<psi>)\<close> by auto
+        with gamma have \<open>\<exists>\<gamma>\<in>snd ?M'. \<Turnstile>\<^sub>P (\<gamma> \<^bold>\<longrightarrow> \<Phi>)\<close> by auto
         ultimately show \<open>the (\<M> ?a M) \<Turnstile>\<^sub>M ?\<psi>\<close> using aM by simp
       qed
     qed
@@ -587,8 +590,8 @@ next
         proof
           assume pre: \<open>M \<Turnstile>\<^sub>M \<phi>' \<and> M \<Turnstile>\<^sub>E (enabledb a)\<close>
           moreover from rImp have \<open>M \<Turnstile>\<^sub>M \<phi> \<and> M \<Turnstile>\<^sub>E (enabledb a) \<longrightarrow> the (\<M> a M) \<Turnstile>\<^sub>M \<psi>\<close> 
-            using \<open>\<nabla>M\<close> transfer_semantics\<^sub>M semantics\<^sub>H.simps(1) semantics\<^sub>P.simps(5) by blast
-          moreover from soundness\<^sub>M  have \<open>M \<Turnstile>\<^sub>M \<phi>' \<^bold>\<longrightarrow> \<phi>\<close> 
+            using \<open>\<nabla>M\<close> transfer_semantics\<^sub>M semantics\<^sub>H.simps(1) semantics\<^sub>P.simps(6) by blast
+          moreover from soundness\<^sub>M  have \<open>M \<Turnstile>\<^sub>M \<phi>' \<^bold>\<longrightarrow> \<phi>\<close>  
             using \<open>\<nabla>M\<close> rImp(1) by blast
           moreover have \<open>\<nabla> (the (\<M> a M))\<close> using \<open>\<nabla>M\<close> \<M>_preserves_mst pre by (cases M) simp
           with soundness\<^sub>M  have \<open>the (\<M> a M) \<Turnstile>\<^sub>M \<psi> \<^bold>\<longrightarrow> \<psi>'\<close> using rImp(4) by blast
@@ -598,7 +601,7 @@ next
         proof
           assume pre: \<open>M \<Turnstile>\<^sub>M \<phi>' \<and> M \<Turnstile>\<^sub>E \<^bold>\<not>(enabledb a)\<close>
           from rImp(3) have \<open>M \<Turnstile>\<^sub>M \<phi> \<and> M \<Turnstile>\<^sub>E \<^bold>\<not>(enabledb a) \<longrightarrow> M \<Turnstile>\<^sub>M \<psi>\<close> 
-            using \<open>\<nabla>M\<close> transfer_semantics\<^sub>M semantics\<^sub>H.simps(1) semantics\<^sub>P.simps(5) by blast
+            using \<open>\<nabla>M\<close> transfer_semantics\<^sub>M semantics\<^sub>H.simps(1) semantics\<^sub>P.simps(6) by blast
           moreover from soundness\<^sub>M  have \<open>M \<Turnstile>\<^sub>M \<phi>' \<^bold>\<longrightarrow> \<phi>\<close> 
             using \<open>\<nabla>M\<close> rImp(1) by blast
           moreover from soundness\<^sub>M  have \<open>M \<Turnstile>\<^sub>M \<psi> \<^bold>\<longrightarrow> \<psi>'\<close>
@@ -630,18 +633,18 @@ next
         proof
           assume \<open>M \<Turnstile>\<^sub>M (\<phi>\<^sub>1 \<^bold>\<or> \<phi>\<^sub>2) \<and> M \<Turnstile>\<^sub>E (enabledb a)\<close> 
           moreover from rDis(2) have \<open>M \<Turnstile>\<^sub>M \<phi>\<^sub>1 \<and> M \<Turnstile>\<^sub>E (enabledb a) \<longrightarrow> the (\<M> a M) \<Turnstile>\<^sub>M \<psi>\<close>
-            using \<open>\<nabla>M\<close> transfer_semantics\<^sub>M semantics\<^sub>H.simps(1) semantics\<^sub>P.simps(5) by blast
+            using \<open>\<nabla>M\<close> transfer_semantics\<^sub>M semantics\<^sub>H.simps(1) semantics\<^sub>P.simps(6) by blast
           moreover from rDis(4) have \<open>M \<Turnstile>\<^sub>M \<phi>\<^sub>2 \<and> M \<Turnstile>\<^sub>E (enabledb a) \<longrightarrow> the (\<M> a M) \<Turnstile>\<^sub>M \<psi>\<close>
-            using \<open>\<nabla>M\<close> transfer_semantics\<^sub>M semantics\<^sub>H.simps(1) semantics\<^sub>P.simps(5) by blast
+            using \<open>\<nabla>M\<close> transfer_semantics\<^sub>M semantics\<^sub>H.simps(1) semantics\<^sub>P.simps(6) by blast
           ultimately show \<open>the (\<M> a M) \<Turnstile>\<^sub>M \<psi>\<close> by auto
         qed
         show \<open>M \<Turnstile>\<^sub>M (\<phi>\<^sub>1 \<^bold>\<or> \<phi>\<^sub>2) \<and> M \<Turnstile>\<^sub>E \<^bold>\<not>(enabledb a) \<longrightarrow> M \<Turnstile>\<^sub>M \<psi>\<close>
         proof
           assume \<open>M \<Turnstile>\<^sub>M (\<phi>\<^sub>1 \<^bold>\<or> \<phi>\<^sub>2) \<and> M \<Turnstile>\<^sub>E \<^bold>\<not>(enabledb a)\<close> 
           moreover from rDis(2) have \<open>M \<Turnstile>\<^sub>M \<phi>\<^sub>1 \<and> M \<Turnstile>\<^sub>E \<^bold>\<not>(enabledb a) \<longrightarrow> M \<Turnstile>\<^sub>M \<psi>\<close>
-            using \<open>\<nabla>M\<close> transfer_semantics\<^sub>M semantics\<^sub>H.simps(1) semantics\<^sub>P.simps(5) by blast
+            using \<open>\<nabla>M\<close> transfer_semantics\<^sub>M semantics\<^sub>H.simps(1) semantics\<^sub>P.simps(6) by blast
           moreover from rDis(4) have \<open>M \<Turnstile>\<^sub>M \<phi>\<^sub>2 \<and> M \<Turnstile>\<^sub>E \<^bold>\<not>(enabledb a) \<longrightarrow> M \<Turnstile>\<^sub>M \<psi>\<close>
-            using \<open>\<nabla>M\<close> transfer_semantics\<^sub>M semantics\<^sub>H.simps(1) semantics\<^sub>P.simps(5) by blast
+            using \<open>\<nabla>M\<close> transfer_semantics\<^sub>M semantics\<^sub>H.simps(1) semantics\<^sub>P.simps(6) by blast
           ultimately show \<open>M \<Turnstile>\<^sub>M \<psi>\<close> by auto
         qed
       qed
@@ -651,4 +654,45 @@ next
 qed auto
 
 end
+
+lemma is_ht_spec_single_agent_program:
+  assumes \<open>\<Pi> \<noteq> {} \<and> \<nabla> M\<close>
+      and \<open>is_ht_specification S\<close>
+      and \<open>\<forall>a. (\<exists>\<phi>. (\<phi>, basic a) \<in> \<Pi>) \<longleftrightarrow> a \<in> set (map fst S)\<close>
+    shows \<open>single_agent_program (SOME \<T>. complies S \<T>) \<Pi> M S\<close> (is \<open>single_agent_program ?\<T> \<Pi> M S\<close>) 
+proof -                     
+  from assms(2) have c: \<open>complies S ?\<T>\<close> using model_exists by (simp add: someI2_ex)
+  moreover have \<open>single_agent ?\<T> \<Pi> M\<close>
+  proof
+    fix a \<Sigma> \<Gamma>
+    show \<open>(\<exists>\<phi>. (\<phi>, basic a) \<in> \<Pi>) \<longrightarrow> \<not> \<Sigma> \<^bold>\<Turnstile>\<^sub>P \<^bold>\<bottom> \<longrightarrow> ?\<T> a (\<Sigma>, \<Gamma>) \<noteq> None \<longrightarrow> \<not> the (?\<T> a (\<Sigma>, \<Gamma>)) \<^bold>\<Turnstile>\<^sub>P \<^bold>\<bottom>\<close> 
+    proof
+      assume \<open>\<exists>\<phi>. (\<phi>, basic a) \<in> \<Pi>\<close>
+      with assms(3) have a: \<open>a \<in> set (map fst S)\<close> by simp
+      then obtain \<Phi> hts where \<open>(a, \<Phi>, hts) \<in> set S\<close> by auto
+      with assms(2) have \<open>complies_hts (a, \<Phi>, hts) ?\<T>\<close> using c unfolding complies_def by simp
+      have \<open>\<forall>ht\<in>set hts. \<not> \<Sigma> \<^bold>\<Turnstile>\<^sub>P \<^bold>\<bottom> \<longrightarrow> ?\<T> a (\<Sigma>, \<Gamma>) \<noteq> None \<longrightarrow> \<not>the (?\<T> a (\<Sigma>, \<Gamma>)) \<^bold>\<Turnstile>\<^sub>P \<^bold>\<bottom>\<close>
+      proof
+        fix ht
+        assume \<open>ht \<in> set hts\<close>
+        with \<open>complies_hts (a, \<Phi>, hts) ?\<T>\<close> have \<open>complies_ht (\<Sigma>, \<Gamma>) ?\<T> \<Phi> (the (htb_basic_unpack ht))\<close> 
+          (is \<open>complies_ht (\<Sigma>, \<Gamma>) ?\<T> \<Phi> ?ht\<close>)
+          unfolding complies_hts_def by simp
+        then have \<open>complies_ht (\<Sigma>, \<Gamma>) ?\<T> \<Phi> (fst ?ht, fst (snd ?ht), snd (snd ?ht))\<close> by simp
+        then have \<open>(\<not> fst (\<Sigma>, \<Gamma>) \<^bold>\<Turnstile>\<^sub>P \<^bold>\<bottom> \<longrightarrow> ?\<T> (fst (snd ?ht)) (\<Sigma>, \<Gamma>) \<noteq> None \<longrightarrow> \<not>the (?\<T> (fst (snd ?ht)) (\<Sigma>, \<Gamma>)) \<^bold>\<Turnstile>\<^sub>P \<^bold>\<bottom>)\<close> 
+          using complies_ht.simps by blast
+        moreover from assms(2) have \<open>fst (snd (the (htb_basic_unpack ht))) = a\<close> 
+          using \<open>(a, \<Phi>, hts) \<in> set S\<close> \<open>ht \<in> set hts\<close> unfolding is_ht_specification_def by simp
+        ultimately show \<open>\<not> \<Sigma> \<^bold>\<Turnstile>\<^sub>P \<^bold>\<bottom> \<longrightarrow> ?\<T> a (\<Sigma>, \<Gamma>) \<noteq> None \<longrightarrow> \<not>the (?\<T> a (\<Sigma>, \<Gamma>)) \<^bold>\<Turnstile>\<^sub>P \<^bold>\<bottom>\<close> by simp
+      qed
+      with assms(2) show \<open>\<not> \<Sigma> \<^bold>\<Turnstile>\<^sub>P \<^bold>\<bottom> \<longrightarrow> ?\<T> a (\<Sigma>, \<Gamma>) \<noteq> None \<longrightarrow> \<not>the (?\<T> a (\<Sigma>, \<Gamma>)) \<^bold>\<Turnstile>\<^sub>P \<^bold>\<bottom>\<close>
+        using \<open>(a, \<Phi>, hts) \<in> set S\<close> unfolding is_ht_specification_def by auto
+    qed
+    show \<open>?\<T> a (\<Sigma>, \<Gamma>) \<noteq> None \<longrightarrow> (\<exists>\<phi>. (\<phi>, basic a) \<in> \<Pi>)\<close> 
+      using c assms(3) unfolding complies_def by auto                                  
+  qed (simp add: assms(1))
+  ultimately show \<open>single_agent_program ?\<T> \<Pi> M S\<close> 
+    using single_agent_program_axioms.intro single_agent_program.intro by simp  
+qed    
+
 end
