Gvf_Mental_States.thy
@@ -19,18 +19,14 @@ type_synonym mental_state = \<open>(\<Phi>\<^sub>L set \<times> \<Phi>\<^sub>L s
     Not all elements of this type are in fact mental states: a number of restrictions apply.\<close>
 definition is_mental_state :: \<open>mental_state \<Rightarrow> bool\<close> (\<open>\<nabla>\<close>) where
   \<open>\<nabla> M \<equiv> let (\<Sigma>, \<Gamma>) = M in \<comment> \<open>Pattern matching to have variables for belief and goal base.\<close> 
-    \<not> \<Sigma> \<Turnstile>\<^sub>L \<bottom>\<^sub>L \<comment> \<open>\<Sigma> is consistent.\<close>
+    \<not> \<Sigma> \<^bold>\<Turnstile>\<^sub>P \<^bold>\<bottom> \<comment> \<open>\<Sigma> is consistent.\<close>
       \<and> (\<forall>\<gamma>\<in>\<Gamma>. \<comment> \<open>for all goals \<gamma> \<in> \<Gamma>:\<close>
-        \<not> \<Sigma> \<Turnstile>\<^sub>L \<gamma> \<comment> \<open>(i) \<gamma> is not entailed by the agent's beliefs,\<close> 
-        \<and> \<not> {} \<Turnstile>\<^sub>L \<^bold>\<not> \<gamma>)\<close> \<comment> \<open>(ii) \<gamma> is consistent.\<close>
+        \<not> \<Sigma> \<^bold>\<Turnstile>\<^sub>P \<gamma> \<comment> \<open>(i) \<gamma> is not entailed by the agent's beliefs,\<close> 
+        \<and> \<not> \<Turnstile>\<^sub>P (\<^bold>\<not> \<gamma>))\<close> \<comment> \<open>(ii) \<gamma> is consistent.\<close>
 \<comment> \<open>Note that the subgoal property for goals is missing. It will be defined in the semantics.\<close>
 
-\<comment> \<open>If \<gamma>' is weaker than a consistent formula \<gamma>, it must itself be consistent.\<close>
-lemma \<open>\<not> {} \<Turnstile>\<^sub>L \<^bold>\<not> \<gamma> \<longrightarrow> {} \<Turnstile>\<^sub>L \<gamma> \<^bold>\<longrightarrow> \<gamma>' \<longrightarrow> \<not> {} \<Turnstile>\<^sub>L \<^bold>\<not> \<gamma>'\<close>
-  by force
-
 \<comment> \<open>Every member (of the goal set) must be weaker than \<bottom>, but not weaker than any belief \<sigma>.\<close>
-lemma \<open>\<nabla> (\<Sigma>, \<Gamma>) \<longrightarrow> (\<forall>\<gamma>\<in>\<Gamma>. {} \<Turnstile>\<^sub>L \<bottom>\<^sub>L \<^bold>\<longrightarrow> \<gamma> \<and> \<not> (\<exists>\<sigma>\<in>\<Sigma>. {} \<Turnstile>\<^sub>L \<sigma> \<^bold>\<longrightarrow> \<gamma>))\<close>
+lemma \<open>\<nabla> (\<Sigma>, \<Gamma>) \<longrightarrow> (\<forall>\<gamma>\<in>\<Gamma>. \<Turnstile>\<^sub>P (\<^bold>\<bottom> \<^bold>\<longrightarrow> \<gamma>) \<and> \<not> (\<exists>\<sigma>\<in>\<Sigma>. \<Turnstile>\<^sub>P (\<sigma> \<^bold>\<longrightarrow> \<gamma>)))\<close>  
   unfolding is_mental_state_def by fastforce
 
 section \<open>Syntax of mental state formulas\<close>
@@ -39,38 +35,33 @@ section \<open>Syntax of mental state formulas\<close>
 datatype Atom\<^sub>M = Bl \<Phi>\<^sub>L | Gl \<Phi>\<^sub>L
 \<comment> \<open>We now use a more complex type for atoms compared to simply natural numbers.
     Bl and Gl are the constructors taking a propositional logic formula as input.
-    We will introduce a nicer syntax below that hides the nested constructors.\<close>
+    We introduce a nicer syntax below that hides the nesting of constructors.\<close>
 
 \<comment> \<open>We set up a type for mental state formulas.\<close>
 type_synonym \<Phi>\<^sub>M = \<open>Atom\<^sub>M \<Phi>\<^sub>P\<close>
 \<comment> \<open>We instantiate the general logic parsing the type for atoms.\<close>
 
-\<comment> \<open>We introduce syntax translations that hide the nesting in the notation.\<close>
-syntax
-  "_B" :: \<open>\<Phi>\<^sub>L \<Rightarrow> \<Phi>\<^sub>M\<close>  (\<open>B _\<close> 55)
-  "_G" :: \<open>\<Phi>\<^sub>L \<Rightarrow> \<Phi>\<^sub>M\<close>  (\<open>G _\<close> 55)
-translations
-  "B \<Phi>" \<rightharpoonup> "(Gvf_Logic.Atom (Atom\<^sub>M.Bl \<Phi>))"
-  "G \<Phi>" \<rightharpoonup> "(Gvf_Logic.Atom (Atom\<^sub>M.Gl \<Phi>))"
-
-\<comment> \<open>Again truth and falsity are defined for this instance of the logic from a simple tautology.\<close>
-abbreviation Truth\<^sub>M :: \<open>\<Phi>\<^sub>M\<close> (\<open>\<top>\<^sub>M\<close>) where 
-  \<open>\<top>\<^sub>M \<equiv> \<^bold>\<not> (B (Atom 0)) \<^bold>\<or> (B (Atom 0))\<close>
-abbreviation Falsity\<^sub>L :: \<open>\<Phi>\<^sub>M\<close> (\<open>\<bottom>\<^sub>M\<close>) where 
-  \<open>\<bottom>\<^sub>M \<equiv> \<^bold>\<not> \<top>\<^sub>M\<close>
+abbreviation \<open>B \<Phi> \<equiv> Atom (Bl \<Phi>)\<close>
+abbreviation \<open>G \<Phi> \<equiv> Atom (Gl \<Phi>)\<close>
 
 section \<open>Semantics\<close>
 
 \<comment> \<open>Semantics of atoms for mental state formulas is derived given a mental state.\<close>
 fun semantics\<^sub>M' :: \<open>mental_state \<Rightarrow> Atom\<^sub>M \<Rightarrow> bool\<close> where
 \<comment> \<open>Does the belief base entail \<Phi>?\<close>
-  \<open>semantics\<^sub>M' (\<Sigma>, _) (Bl \<Phi>) = (\<Sigma> \<Turnstile>\<^sub>L \<Phi>)\<close> |
+  \<open>semantics\<^sub>M' (\<Sigma>, _) (Bl \<Phi>) = (\<Sigma> \<^bold>\<Turnstile>\<^sub>P \<Phi>)\<close> |
 \<comment> \<open>Is \<Phi> not entailed by the belief base and a (sub)goal?\<close>
-  \<open>semantics\<^sub>M' (\<Sigma>, \<Gamma>) (Gl \<Phi>) = (\<not> \<Sigma> \<Turnstile>\<^sub>L \<Phi> \<and> (\<exists>\<gamma>\<in>\<Gamma>. {} \<Turnstile>\<^sub>L \<gamma> \<^bold>\<longrightarrow> \<Phi>))\<close>
+  \<open>semantics\<^sub>M' (\<Sigma>, \<Gamma>) (Gl \<Phi>) = (\<not> \<Sigma> \<^bold>\<Turnstile>\<^sub>P \<Phi> \<and> (\<exists>\<gamma>\<in>\<Gamma>. \<Turnstile>\<^sub>P (\<gamma> \<^bold>\<longrightarrow> \<Phi>)))\<close>
 
 \<comment> \<open>Semantics of formulas.\<close>
 abbreviation semantics\<^sub>M :: \<open>mental_state \<Rightarrow> \<Phi>\<^sub>M \<Rightarrow> bool\<close> (infix \<open>\<Turnstile>\<^sub>M\<close> 50) where
   \<open>M \<Turnstile>\<^sub>M \<phi> \<equiv> semantics\<^sub>P (semantics\<^sub>M' M) \<phi>\<close>
+\<comment> \<open>The semantics for atoms, given a mental state, matches the type for an interpretation.
+    The curried function is parsed on to the general semantics as an interpretation which allows
+    reuse of the existing definition.\<close>
+
+abbreviation semantics\<^sub>_all\<^sub>M :: \<open>\<Phi>\<^sub>M \<Rightarrow> bool\<close> (\<open>\<^bold>\<Turnstile>\<^sub>M\<close>) where
+  \<open>\<^bold>\<Turnstile>\<^sub>M \<phi> \<equiv> (\<forall>M. semantics\<^sub>P (semantics\<^sub>M' M) \<phi>)\<close>
 \<comment> \<open>The semantics for atoms, given a mental state, matches the type for an interpretation.
     The curried function is parsed on to the general semantics as an interpretation which allows
     reuse of the existing definition.\<close>
@@ -81,9 +72,9 @@ lemma \<open>({ \<Phi> }, {}) \<Turnstile>\<^sub>M B \<Phi>\<close> by simp
 lemma \<open>({ Atom 0 }, { Atom 2 }) \<Turnstile>\<^sub>M G (Atom 1 \<^bold>\<longrightarrow> Atom 2)\<close> (is \<open>({ ?R }, { ?Q }) \<Turnstile>\<^sub>M G (?P \<^bold>\<longrightarrow> ?Q)\<close>)
 proof -
   have \<open>?R \<noteq> ?Q\<close> by simp
-  have \<open>\<not> { ?R } \<Turnstile>\<^sub>P ?P \<^bold>\<longrightarrow> ?Q\<close>
+  have \<open>\<not> { ?R } \<^bold>\<Turnstile>\<^sub>P ?P \<^bold>\<longrightarrow> ?Q\<close>
   proof 
-    assume \<open>{ ?R } \<Turnstile>\<^sub>P ?P \<^bold>\<longrightarrow> ?Q\<close>
+    assume \<open>{ ?R } \<^bold>\<Turnstile>\<^sub>P ?P \<^bold>\<longrightarrow> ?Q\<close>
     then have \<open>\<forall>f. semantics\<^sub>P f ?R \<longrightarrow> semantics\<^sub>P f (?P \<^bold>\<longrightarrow> ?Q)\<close> by auto
     moreover have \<open>\<exists>f. \<not> (semantics\<^sub>P f ?R \<longrightarrow> semantics\<^sub>P f (?P \<^bold>\<longrightarrow> ?Q))\<close>
     proof
@@ -92,93 +83,96 @@ proof -
     qed
     ultimately show False by auto
   qed
-  then have \<open>\<not> { Atom 0 } \<Turnstile>\<^sub>L (Atom 1 \<^bold>\<longrightarrow> Atom 2)\<close> by simp
-  moreover have \<open>{} \<Turnstile>\<^sub>L Atom 2 \<^bold>\<longrightarrow> (Atom 1 \<^bold>\<longrightarrow> Atom 2)\<close> by simp
-  then have \<open>\<exists>\<gamma>\<in>{ Atom 2 }. {} \<Turnstile>\<^sub>L \<gamma> \<^bold>\<longrightarrow> (Atom 1 \<^bold>\<longrightarrow> Atom 2)\<close> by simp
+  then have \<open>\<not> { Atom (0::nat) } \<^bold>\<Turnstile>\<^sub>P (Atom 1 \<^bold>\<longrightarrow> Atom 2)\<close> by simp
+  moreover have \<open>\<Turnstile>\<^sub>P (Atom 2 \<^bold>\<longrightarrow> (Atom 1 \<^bold>\<longrightarrow> Atom 2))\<close> by simp
+  then have \<open>\<exists>\<gamma>\<in>{ Atom 2 }. \<Turnstile>\<^sub>P (\<gamma> \<^bold>\<longrightarrow> (Atom 1 \<^bold>\<longrightarrow> Atom 2))\<close> by simp
   ultimately show ?thesis by simp
 qed
 
 section \<open>Various proofs\<close>
 
 \<comment> \<open>An agent cannot have a goal to achieve a tautology.\<close>
-lemma \<open>\<nabla> M \<longrightarrow> \<not> M \<Turnstile>\<^sub>M G \<top>\<^sub>L\<close> 
+lemma \<open>\<nabla> M \<longrightarrow> \<not> M \<Turnstile>\<^sub>M G \<^bold>\<top>\<close> 
   unfolding is_mental_state_def by auto
 
 \<comment> \<open>An agent does not have inconsistent beliefs/goals.\<close>
-lemma not_modal_False: \<open>\<nabla> M \<longrightarrow> M \<Turnstile>\<^sub>M \<^bold>\<not> (B \<bottom>\<^sub>L)\<close> \<open>\<nabla> M \<longrightarrow> M \<Turnstile>\<^sub>M \<^bold>\<not> (G \<bottom>\<^sub>L)\<close>
+lemma not_modal_False: \<open>\<nabla> M \<longrightarrow> M \<Turnstile>\<^sub>M \<^bold>\<not> (B \<^bold>\<bottom>)\<close> \<open>\<nabla> M \<longrightarrow> M \<Turnstile>\<^sub>M \<^bold>\<not> (G \<^bold>\<bottom>)\<close>
   unfolding is_mental_state_def by fastforce+
+
+lemma bel_dist_conj: \<open>M \<Turnstile>\<^sub>M B (\<phi> \<^bold>\<and> \<psi>) \<longleftrightarrow> M \<Turnstile>\<^sub>M B \<phi> \<and> M \<Turnstile>\<^sub>M B \<psi>\<close>
+  using semantics\<^sub>M'.elims(2) by fastforce
 
 \<comment> \<open>Properties of the goal modality.\<close>
 lemma G_properties:
-  shows \<open>\<not> (\<forall>\<Sigma> \<Gamma> \<Phi> \<psi>. \<nabla> (\<Sigma>, \<Gamma>) \<longrightarrow> (\<Sigma>, \<Gamma>) \<Turnstile>\<^sub>M (G \<Phi> \<^bold>\<longrightarrow> \<psi>) \<^bold>\<longrightarrow> (G \<Phi>) \<^bold>\<longrightarrow> (G \<psi>))\<close>
-    and \<open>\<not> (\<forall>\<Sigma> \<Gamma> \<Phi> \<psi>. \<nabla> (\<Sigma>, \<Gamma>) \<longrightarrow> (\<Sigma>, \<Gamma>) \<Turnstile>\<^sub>M (G \<Phi> \<^bold>\<and> (\<Phi> \<^bold>\<longrightarrow> \<psi>)) \<^bold>\<longrightarrow> (G \<psi>))\<close>
-    and \<open>\<not> (\<forall>\<Sigma> \<Gamma> \<Phi> \<psi>. \<nabla> (\<Sigma>, \<Gamma>) \<longrightarrow> (\<Sigma>, \<Gamma>) \<Turnstile>\<^sub>M (G \<Phi>) \<^bold>\<and> (G \<psi>) \<^bold>\<longrightarrow> (G \<Phi> \<^bold>\<and> \<psi>))\<close>
-    and \<open>{} \<Turnstile>\<^sub>L \<Phi> \<^bold>\<longleftrightarrow> \<psi> \<longrightarrow> \<nabla> (\<Sigma>, \<Gamma>) \<longrightarrow> (\<Sigma>, \<Gamma>) \<Turnstile>\<^sub>M (G \<Phi>) \<^bold>\<longleftrightarrow> (G \<psi>)\<close>
+  shows \<open>\<not> (\<forall>\<Sigma> \<Gamma> \<Phi> \<psi>. \<nabla> (\<Sigma>, \<Gamma>) \<longrightarrow> (\<Sigma>, \<Gamma>) \<Turnstile>\<^sub>M G (\<Phi> \<^bold>\<longrightarrow> \<psi>) \<^bold>\<longrightarrow> G \<Phi> \<^bold>\<longrightarrow> G \<psi>)\<close>
+    and \<open>\<not> (\<forall>\<Sigma> \<Gamma> \<Phi> \<psi>. \<nabla> (\<Sigma>, \<Gamma>) \<longrightarrow> (\<Sigma>, \<Gamma>) \<Turnstile>\<^sub>M G (\<Phi> \<^bold>\<and> (\<Phi> \<^bold>\<longrightarrow> \<psi>)) \<^bold>\<longrightarrow> G \<psi>)\<close>
+    and \<open>\<not> (\<forall>\<Sigma> \<Gamma> \<Phi> \<psi>. \<nabla> (\<Sigma>, \<Gamma>) \<longrightarrow> (\<Sigma>, \<Gamma>) \<Turnstile>\<^sub>M G \<Phi> \<^bold>\<and> G \<psi> \<^bold>\<longrightarrow> G (\<Phi> \<^bold>\<and> \<psi>))\<close>
+    and \<open>\<Turnstile>\<^sub>P (\<Phi> \<^bold>\<longleftrightarrow> \<psi>) \<longrightarrow> \<nabla> (\<Sigma>, \<Gamma>) \<longrightarrow> (\<Sigma>, \<Gamma>) \<Turnstile>\<^sub>M G \<Phi> \<^bold>\<longleftrightarrow> G \<psi>\<close>
 proof -
-  let ?\<psi> = \<open>Atom 0\<close> and
-      ?\<Phi> = \<open>Atom 1\<close>
-  show \<open>\<not> (\<forall>\<Sigma> \<Gamma> \<Phi> \<psi>. \<nabla> (\<Sigma>, \<Gamma>) \<longrightarrow> (\<Sigma>, \<Gamma>) \<Turnstile>\<^sub>M (G (\<Phi> \<^bold>\<longrightarrow> \<psi>)) \<^bold>\<longrightarrow> (G \<Phi>) \<^bold>\<longrightarrow> (G \<psi>))\<close>
+  let ?\<Phi> = \<open>Atom (0::nat)\<close> and ?\<psi> = \<open>Atom (1::nat)\<close>
+  show \<open>\<not> (\<forall>\<Sigma> \<Gamma> \<Phi> \<psi>. \<nabla> (\<Sigma>, \<Gamma>) \<longrightarrow> (\<Sigma>, \<Gamma>) \<Turnstile>\<^sub>M G (\<Phi> \<^bold>\<longrightarrow> \<psi>) \<^bold>\<longrightarrow> G \<Phi> \<^bold>\<longrightarrow> G \<psi>)\<close>
   proof 
-    assume *: \<open>\<forall>\<Sigma> \<Gamma> \<Phi> \<psi>. \<nabla> (\<Sigma>, \<Gamma>) \<longrightarrow> (\<Sigma>, \<Gamma>) \<Turnstile>\<^sub>M (G \<Phi> \<^bold>\<longrightarrow> \<psi>) \<^bold>\<longrightarrow> (G \<Phi>) \<^bold>\<longrightarrow> (G \<psi>)\<close>
+    assume *: \<open>\<forall>\<Sigma> \<Gamma> \<Phi> \<psi>. \<nabla> (\<Sigma>, \<Gamma>) \<longrightarrow> (\<Sigma>, \<Gamma>) \<Turnstile>\<^sub>M G (\<Phi> \<^bold>\<longrightarrow> \<psi>) \<^bold>\<longrightarrow> G \<Phi> \<^bold>\<longrightarrow> G \<psi>\<close> 
     \<comment> \<open>Counter example.\<close>
-    let ?\<Sigma> = \<open>{}\<close> and ?\<Gamma> = \<open>{ ?\<Phi> \<^bold>\<longrightarrow> ?\<psi>, ?\<Phi> }\<close>
-    have \<open>\<not> (?\<Sigma>, ?\<Gamma>) \<Turnstile>\<^sub>M (G ?\<Phi> \<^bold>\<longrightarrow> ?\<psi>) \<^bold>\<longrightarrow> (G ?\<Phi>) \<^bold>\<longrightarrow> (G ?\<psi>)\<close> by auto
-    moreover have \<open>\<nabla> (?\<Sigma>, ?\<Gamma>)\<close> unfolding is_mental_state_def by auto
-    ultimately show False using * by blast      
+    moreover have \<open>\<exists>\<Sigma> \<Gamma> \<Phi> \<psi>. \<nabla> (\<Sigma>, \<Gamma>) \<and> \<not> (\<Sigma>, \<Gamma>) \<Turnstile>\<^sub>M G (\<Phi> \<^bold>\<longrightarrow> \<psi>) \<^bold>\<longrightarrow> G \<Phi> \<^bold>\<longrightarrow> G \<psi>\<close>
+    proof -
+      let ?\<Sigma> = \<open>{}\<close> and ?\<Gamma> = \<open>{ ?\<Phi> \<^bold>\<longrightarrow> ?\<psi>, ?\<Phi> }\<close>
+      have \<open>\<not> (?\<Sigma>, ?\<Gamma>) \<Turnstile>\<^sub>M G (?\<Phi> \<^bold>\<longrightarrow> ?\<psi>) \<^bold>\<longrightarrow> G ?\<Phi> \<^bold>\<longrightarrow> G ?\<psi>\<close> by auto
+      moreover have \<open>\<nabla> (?\<Sigma>, ?\<Gamma>)\<close> unfolding is_mental_state_def by auto
+      ultimately show ?thesis by blast
+    qed
+    ultimately show False by blast
   qed
-  show \<open>\<not> (\<forall>\<Sigma> \<Gamma> \<Phi> \<psi>. \<nabla> (\<Sigma>, \<Gamma>) \<longrightarrow> (\<Sigma>, \<Gamma>) \<Turnstile>\<^sub>M (G \<Phi> \<^bold>\<and> (\<Phi> \<^bold>\<longrightarrow> \<psi>)) \<^bold>\<longrightarrow> (G \<psi>))\<close>
+  show \<open>\<not> (\<forall>\<Sigma> \<Gamma> \<Phi> \<psi>. \<nabla> (\<Sigma>, \<Gamma>) \<longrightarrow> (\<Sigma>, \<Gamma>) \<Turnstile>\<^sub>M G (\<Phi> \<^bold>\<and> (\<Phi> \<^bold>\<longrightarrow> \<psi>)) \<^bold>\<longrightarrow> G \<psi>)\<close>
   proof
-    assume *: \<open>\<forall>\<Sigma> \<Gamma> \<Phi> \<psi>. \<nabla> (\<Sigma>, \<Gamma>) \<longrightarrow> (\<Sigma>, \<Gamma>) \<Turnstile>\<^sub>M (G \<Phi> \<^bold>\<and> (\<Phi> \<^bold>\<longrightarrow> \<psi>)) \<^bold>\<longrightarrow> (G \<psi>)\<close>
+    assume *: \<open>\<forall>\<Sigma> \<Gamma> \<Phi> \<psi>. \<nabla> (\<Sigma>, \<Gamma>) \<longrightarrow> (\<Sigma>, \<Gamma>) \<Turnstile>\<^sub>M G (\<Phi> \<^bold>\<and> (\<Phi> \<^bold>\<longrightarrow> \<psi>)) \<^bold>\<longrightarrow> G \<psi>\<close>
     \<comment> \<open>Counter example.\<close>
     let ?\<Sigma> = \<open>{ ?\<psi> }\<close> and ?\<Gamma> = \<open>{ ?\<Phi> \<^bold>\<and> (?\<Phi> \<^bold>\<longrightarrow> ?\<psi>) }\<close>
-    have \<open>\<not> (?\<Sigma>, ?\<Gamma>) \<Turnstile>\<^sub>M (G ?\<Phi> \<^bold>\<and> (?\<Phi> \<^bold>\<longrightarrow> ?\<psi>)) \<^bold>\<longrightarrow> (G ?\<psi>)\<close>
-      by auto
+    have \<open>\<not> (?\<Sigma>, ?\<Gamma>) \<Turnstile>\<^sub>M G (?\<Phi> \<^bold>\<and> (?\<Phi> \<^bold>\<longrightarrow> ?\<psi>)) \<^bold>\<longrightarrow> G ?\<psi>\<close> by auto
     moreover have \<open>\<nabla> (?\<Sigma>, ?\<Gamma>)\<close> unfolding is_mental_state_def by auto
     ultimately show False using * by blast
-    qed
-  show \<open>\<not> (\<forall>\<Sigma> \<Gamma> \<Phi> \<psi>. \<nabla> (\<Sigma>, \<Gamma>) \<longrightarrow> (\<Sigma>, \<Gamma>) \<Turnstile>\<^sub>M (G \<Phi>) \<^bold>\<and> (G \<psi>) \<^bold>\<longrightarrow> (G \<Phi> \<^bold>\<and> \<psi>))\<close>
+  qed
+  show \<open>\<not> (\<forall>\<Sigma> \<Gamma> \<Phi> \<psi>. \<nabla> (\<Sigma>, \<Gamma>) \<longrightarrow> (\<Sigma>, \<Gamma>) \<Turnstile>\<^sub>M G \<Phi> \<^bold>\<and> G \<psi> \<^bold>\<longrightarrow> G (\<Phi> \<^bold>\<and> \<psi>))\<close>
   proof
-    assume *: \<open>\<forall>\<Sigma> \<Gamma> \<Phi> \<psi>. \<nabla> (\<Sigma>, \<Gamma>) \<longrightarrow> (\<Sigma>, \<Gamma>) \<Turnstile>\<^sub>M (G \<Phi>) \<^bold>\<and> (G \<psi>) \<^bold>\<longrightarrow> (G \<Phi> \<^bold>\<and> \<psi>)\<close>
+    assume *: \<open>\<forall>\<Sigma> \<Gamma> \<Phi> \<psi>. \<nabla> (\<Sigma>, \<Gamma>) \<longrightarrow> (\<Sigma>, \<Gamma>) \<Turnstile>\<^sub>M (G \<Phi>) \<^bold>\<and> (G \<psi>) \<^bold>\<longrightarrow> G (\<Phi> \<^bold>\<and> \<psi>)\<close>
     \<comment> \<open>Counter example.\<close>
     let ?\<Sigma> = \<open>{}\<close> and 
         ?\<Gamma> = \<open>{ ?\<Phi>, ?\<psi> }\<close>
-    have \<open>\<not> (?\<Sigma>, ?\<Gamma>) \<Turnstile>\<^sub>M (G ?\<Phi>) \<^bold>\<and> (G ?\<psi>) \<^bold>\<longrightarrow> (G ?\<Phi> \<^bold>\<and> ?\<psi>)\<close>
+    have \<open>\<not> (?\<Sigma>, ?\<Gamma>) \<Turnstile>\<^sub>M (G ?\<Phi>) \<^bold>\<and> (G ?\<psi>) \<^bold>\<longrightarrow> G (?\<Phi> \<^bold>\<and> ?\<psi>)\<close>
       by auto
     moreover have \<open>\<nabla> (?\<Sigma>, ?\<Gamma>)\<close>
       unfolding is_mental_state_def by auto
     ultimately show False 
       using * by blast
   qed
-  show \<open>{} \<Turnstile>\<^sub>L \<Phi> \<^bold>\<longleftrightarrow> \<psi> \<longrightarrow> \<nabla> (\<Sigma>, \<Gamma>) \<longrightarrow> (\<Sigma>, \<Gamma>) \<Turnstile>\<^sub>M (G \<Phi>) \<^bold>\<longleftrightarrow> (G \<psi>)\<close>
-    by simp
-qed
+qed simp
 
 section \<open>Provability\<close>
 
 \<comment> \<open>A proof system for mental state formulas.\<close>
 inductive derive\<^sub>M :: \<open>\<Phi>\<^sub>M \<Rightarrow> bool\<close> (\<open>\<turnstile>\<^sub>M _\<close> 40) where
   \<comment> \<open>Derive classical tautologies.\<close>
-  R1: \<open>\<turnstile>\<^sub>P \<phi> \<Longrightarrow> \<turnstile>\<^sub>M \<phi>\<close> |
+  R1: \<open>\<Turnstile>\<^sub>P \<phi> \<Longrightarrow> \<turnstile>\<^sub>M \<phi>\<close> |
   \<comment> \<open>Properties of beliefs.\<close> 
-  R2: \<open>\<turnstile>\<^sub>P \<Phi> \<Longrightarrow> \<turnstile>\<^sub>M (B \<Phi>)\<close> |
-  A1: \<open>\<turnstile>\<^sub>M ((B \<Phi> \<^bold>\<longrightarrow> \<psi>) \<^bold>\<longrightarrow> (B \<Phi>) \<^bold>\<longrightarrow> (B \<psi>))\<close> |
-  A2: \<open>\<turnstile>\<^sub>M (\<^bold>\<not> (B \<bottom>\<^sub>L))\<close> |
+  R2: \<open>\<Turnstile>\<^sub>P \<Phi> \<Longrightarrow> \<turnstile>\<^sub>M B \<Phi>\<close> |
+  A1: \<open>\<turnstile>\<^sub>M B (\<Phi> \<^bold>\<longrightarrow> \<psi>) \<^bold>\<longrightarrow> B \<Phi> \<^bold>\<longrightarrow> B \<psi>\<close> |
+  A2: \<open>\<turnstile>\<^sub>M \<^bold>\<not> (B \<^bold>\<bottom>)\<close> |
   \<comment> \<open>Properties of goals.\<close>
-  A3: \<open>\<turnstile>\<^sub>M (\<^bold>\<not> (G \<bottom>\<^sub>L))\<close> |
-  A4: \<open>\<turnstile>\<^sub>M ((B \<Phi>) \<^bold>\<longrightarrow> (\<^bold>\<not> (G \<Phi>)))\<close> |
-  A5: \<open>\<turnstile>\<^sub>P (\<Phi> \<^bold>\<longrightarrow> \<psi>) \<Longrightarrow> \<turnstile>\<^sub>M ((\<^bold>\<not> (B \<psi>)) \<^bold>\<longrightarrow> (G \<Phi>) \<^bold>\<longrightarrow> (G \<psi>))\<close>
+  A3: \<open>\<turnstile>\<^sub>M \<^bold>\<not> (G \<^bold>\<bottom>)\<close> |
+  A4: \<open>\<turnstile>\<^sub>M B \<Phi> \<^bold>\<longrightarrow> \<^bold>\<not> (G \<Phi>)\<close> |
+  A5: \<open>\<Turnstile>\<^sub>P (\<Phi> \<^bold>\<longrightarrow> \<psi>) \<Longrightarrow> \<turnstile>\<^sub>M \<^bold>\<not> (B \<psi>) \<^bold>\<longrightarrow> G \<Phi> \<^bold>\<longrightarrow> G \<psi>\<close>
 \<comment> \<open>The original definition uses semantic arguments in e.g. A5. Since we have soundness, but
     not completeness (yet), it may be an idea to switch back. Initially I preferred to keep
     semantics arguments out of the proof system.\<close>
 
 \<comment> \<open>Example.\<close>
-lemma \<open>\<turnstile>\<^sub>M (B \<Phi>) \<^bold>\<or> (\<^bold>\<not> (B \<Phi>))\<close> (is \<open>\<turnstile>\<^sub>M ?P \<^bold>\<or> \<^bold>\<not> ?P\<close>) 
+lemma \<open>\<turnstile>\<^sub>M B \<Phi> \<^bold>\<or> \<^bold>\<not> (B \<Phi>)\<close> (is \<open>\<turnstile>\<^sub>M ?P \<^bold>\<or> \<^bold>\<not> ?P\<close>) 
 proof
   from R_Or have \<open>\<turnstile>\<^sub>P ?P \<^bold>\<or> \<^bold>\<not> ?P\<close> if \<open>{#} \<turnstile>\<^sub>P# {#} + {# ?P, \<^bold>\<not> ?P #}\<close> using that by auto
   with R_Neg have \<open>\<turnstile>\<^sub>P ?P \<^bold>\<or> \<^bold>\<not> ?P\<close> if \<open>{# ?P #} \<turnstile>\<^sub>P# {# ?P #}\<close> using that
     by (metis add_mset_add_single empty_neutral(1) union_commute)
     (* Multiset is giving some problems with single stepping it seems... *)
-  with Axiom show \<open>\<turnstile>\<^sub>P ?P \<^bold>\<or> \<^bold>\<not> ?P\<close> by auto
+  with Axiom show \<open>\<Turnstile>\<^sub>P (?P \<^bold>\<or> \<^bold>\<not> ?P)\<close> by auto
 qed
 
 section \<open>Soundness\<close>
@@ -188,13 +182,13 @@ theorem soundness\<^sub>M:
   assumes \<open>\<nabla> M\<close> 
   shows \<open>\<turnstile>\<^sub>M \<Phi> \<Longrightarrow> M \<Turnstile>\<^sub>M \<Phi>\<close>
 proof (induct rule: derive\<^sub>M.induct)
-  case (R1 \<phi>)
-  with soundness\<^sub>P show ?case by fastforce
+  case R1
+  then show ?case by fastforce
 next
-  case (R2 \<Phi>)
-  with soundness\<^sub>P show ?case by (cases M) fastforce
+  case R2
+  then show ?case by (cases M) fastforce
 next
-  case (A1 \<Phi> \<psi>)
+  case A1
   then show ?case by (cases M) auto
 next
   case A2
@@ -209,31 +203,30 @@ next
   with \<open>\<nabla> M\<close> show ?case unfolding is_mental_state_def by auto
 next
   case (A5 \<Phi> \<psi>)
-  with soundness\<^sub>P have \<open>{} \<Turnstile>\<^sub>L \<Phi> \<^bold>\<longrightarrow> \<psi>\<close> by fastforce
   show ?case
   proof -
-    have \<open>M \<Turnstile>\<^sub>M \<^bold>\<not> (B \<psi>) \<longrightarrow> M \<Turnstile>\<^sub>M (G \<Phi>) \<longrightarrow> M \<Turnstile>\<^sub>M G \<psi>\<close>
+    have \<open>M \<Turnstile>\<^sub>M \<^bold>\<not> (B \<psi>) \<longrightarrow> M \<Turnstile>\<^sub>M G \<Phi> \<longrightarrow> M \<Turnstile>\<^sub>M G \<psi>\<close>
     proof (cases M)
       case (Pair \<Sigma> \<Gamma>)
-      have \<open>(\<Sigma>, \<Gamma>) \<Turnstile>\<^sub>M \<^bold>\<not> (B \<psi>) \<longrightarrow> (\<Sigma>, \<Gamma>) \<Turnstile>\<^sub>M (G \<Phi>) \<longrightarrow> (\<Sigma>, \<Gamma>) \<Turnstile>\<^sub>M G \<psi>\<close>
+      have \<open>(\<Sigma>, \<Gamma>) \<Turnstile>\<^sub>M \<^bold>\<not> (B \<psi>) \<longrightarrow> (\<Sigma>, \<Gamma>) \<Turnstile>\<^sub>M G \<Phi> \<longrightarrow> (\<Sigma>, \<Gamma>) \<Turnstile>\<^sub>M G \<psi>\<close>
       proof
         assume \<open>(\<Sigma>, \<Gamma>) \<Turnstile>\<^sub>M \<^bold>\<not> (B \<psi>)\<close>
-        then have \<open>\<not>\<Sigma> \<Turnstile>\<^sub>L \<psi>\<close> by simp
-        show \<open>(\<Sigma>, \<Gamma>) \<Turnstile>\<^sub>M (G \<Phi>) \<longrightarrow> (\<Sigma>, \<Gamma>) \<Turnstile>\<^sub>M G \<psi>\<close>
+        then have \<open>\<not> \<Sigma> \<^bold>\<Turnstile>\<^sub>P \<psi>\<close> by simp
+        show \<open>(\<Sigma>, \<Gamma>) \<Turnstile>\<^sub>M G \<Phi> \<longrightarrow> (\<Sigma>, \<Gamma>) \<Turnstile>\<^sub>M G \<psi>\<close>
         proof
           assume \<open>(\<Sigma>, \<Gamma>) \<Turnstile>\<^sub>M G \<Phi>\<close>
-          then have \<open>\<Phi>\<in>\<Gamma> \<or> \<not>\<Sigma> \<Turnstile>\<^sub>L \<Phi> \<and> (\<exists>\<gamma>\<in>\<Gamma>. {} \<Turnstile>\<^sub>L \<gamma> \<^bold>\<longrightarrow> \<Phi>)\<close> by simp
+          then have \<open>\<Phi>\<in>\<Gamma> \<or> \<not>\<Sigma> \<^bold>\<Turnstile>\<^sub>P \<Phi> \<and> (\<exists>\<gamma>\<in>\<Gamma>. \<Turnstile>\<^sub>P (\<gamma> \<^bold>\<longrightarrow> \<Phi>))\<close> by simp
           then show \<open>(\<Sigma>, \<Gamma>) \<Turnstile>\<^sub>M G \<psi>\<close> 
           proof
             assume \<open>\<Phi> \<in> \<Gamma>\<close>
-            with \<open>{} \<Turnstile>\<^sub>L \<Phi> \<^bold>\<longrightarrow> \<psi>\<close> have \<open>(\<exists>\<gamma>\<in>\<Gamma>. {} \<Turnstile>\<^sub>L \<gamma> \<^bold>\<longrightarrow> \<psi>)\<close> by auto
-            with \<open>\<not>\<Sigma> \<Turnstile>\<^sub>L \<psi>\<close> show ?thesis by simp
+            with \<open>\<Turnstile>\<^sub>P (\<Phi> \<^bold>\<longrightarrow> \<psi>)\<close> have \<open>\<exists>\<gamma>\<in>\<Gamma>. \<Turnstile>\<^sub>P (\<gamma> \<^bold>\<longrightarrow> \<psi>)\<close> by auto
+            with \<open>\<not>\<Sigma> \<^bold>\<Turnstile>\<^sub>P \<psi>\<close> show ?thesis by simp
           next
-            assume \<open>\<not> \<Sigma> \<Turnstile>\<^sub>L \<Phi> \<and> (\<exists>\<gamma>\<in>\<Gamma>. {} \<Turnstile>\<^sub>L \<gamma> \<^bold>\<longrightarrow> \<Phi>)\<close>
-            then have \<open>\<not> \<Sigma> \<Turnstile>\<^sub>L \<Phi>\<close> \<open>(\<exists>\<gamma>\<in>\<Gamma>. {} \<Turnstile>\<^sub>L \<gamma> \<^bold>\<longrightarrow> \<Phi>)\<close> by simp+
-            from \<open>(\<exists>\<gamma>\<in>\<Gamma>. {} \<Turnstile>\<^sub>L \<gamma> \<^bold>\<longrightarrow> \<Phi>)\<close> have \<open>(\<exists>\<gamma>\<in>\<Gamma>. {} \<Turnstile>\<^sub>L \<gamma> \<^bold>\<longrightarrow> \<psi>)\<close> 
-              using \<open>{} \<Turnstile>\<^sub>L \<Phi> \<^bold>\<longrightarrow> \<psi>\<close> by auto
-            with \<open>\<not> \<Sigma> \<Turnstile>\<^sub>L \<psi>\<close> show ?thesis by simp
+            assume \<open>\<not> \<Sigma> \<^bold>\<Turnstile>\<^sub>P \<Phi> \<and> (\<exists>\<gamma>\<in>\<Gamma>. \<Turnstile>\<^sub>P (\<gamma> \<^bold>\<longrightarrow> \<Phi>))\<close>
+            then have \<open>\<not> \<Sigma> \<^bold>\<Turnstile>\<^sub>P \<Phi>\<close> \<open>\<exists>\<gamma>\<in>\<Gamma>. \<Turnstile>\<^sub>P (\<gamma> \<^bold>\<longrightarrow> \<Phi>)\<close> by simp+
+            from \<open>\<exists>\<gamma>\<in>\<Gamma>. \<Turnstile>\<^sub>P (\<gamma> \<^bold>\<longrightarrow> \<Phi>)\<close> have \<open>\<exists>\<gamma>\<in>\<Gamma>. \<Turnstile>\<^sub>P (\<gamma> \<^bold>\<longrightarrow> \<psi>)\<close> 
+              using \<open>\<Turnstile>\<^sub>P (\<Phi> \<^bold>\<longrightarrow> \<psi>)\<close> by auto
+            with \<open>\<not> \<Sigma> \<^bold>\<Turnstile>\<^sub>P \<psi>\<close> show ?thesis by simp
           qed 
         qed
       qed
