Gvf_Temporal_Logic.thy
@@ -9,7 +9,7 @@ theory Gvf_Temporal_Logic imports Gvf_Agent_Specification begin
 section \<open>Syntax\<close> 
 
 datatype 'a \<Phi>\<^sub>T =
-  Falsity (\<open>\<bottom>\<^sub>T\<close>) |
+  F (\<open>\<bottom>\<^sub>T\<close>) |
   Atom 'a |
   Negation \<open>'a \<Phi>\<^sub>T\<close> (\<open>\<not>\<^sub>T\<close>) | 
   Implication \<open>'a \<Phi>\<^sub>T\<close> \<open>'a \<Phi>\<^sub>T\<close> (infixr \<open>\<longrightarrow>\<^sub>T\<close> 60) | 
@@ -19,7 +19,10 @@ datatype 'a \<Phi>\<^sub>T =
   until \<open>'a \<Phi>\<^sub>T\<close> \<open>'a \<Phi>\<^sub>T\<close> (infix \<open>until\<close> 55)
 
 \<comment> \<open>The type for temporal logic (mental state) formulas including enabledness.\<close>
-type_synonym \<Phi>\<^sub>T\<^sub>E = \<open>Atom\<^sub>E \<Phi>\<^sub>T\<close>
+type_synonym \<Phi>\<^sub>T\<^sub>M = \<open>Atom\<^sub>M \<Phi>\<^sub>T\<close>
+
+abbreviation \<open>B\<^sub>T \<Phi> \<equiv> Atom (Bl \<Phi>)\<close>
+abbreviation \<open>G\<^sub>T \<Phi> \<equiv> Atom (Gl \<Phi>)\<close>
 
 \<comment> \<open>A number of other well known temporal operators can be defined in terms of the operator until.\<close> 
 
@@ -36,6 +39,7 @@ definition unless :: \<open>'a \<Phi>\<^sub>T \<Rightarrow> 'a \<Phi>\<^sub>T \<
 
 fun to_\<Phi>\<^sub>T :: \<open>'a \<Phi>\<^sub>P \<Rightarrow> 'a \<Phi>\<^sub>T\<close> (\<open>_\<^sup>T\<close> [100]) where
   \<open>(\<Phi>\<^sub>P.Atom x)\<^sup>T = Atom x\<close> |
+  \<open>\<^bold>\<bottom>\<^sup>T = \<bottom>\<^sub>T\<close> |
   \<open>(\<^bold>\<not> p)\<^sup>T = (\<not>\<^sub>T (p\<^sup>T))\<close> |
   \<open>(p \<^bold>\<longrightarrow> q)\<^sup>T = (p\<^sup>T \<longrightarrow>\<^sub>T q\<^sup>T)\<close> |
   \<open>(p \<^bold>\<or> q)\<^sup>T = (p\<^sup>T \<or>\<^sub>T q\<^sup>T)\<close> |
@@ -45,9 +49,9 @@ section \<open>Semantics\<close>
 
 context single_agent_program begin
 
-fun semantics\<^sub>T :: \<open>trace \<Rightarrow> nat \<Rightarrow> \<Phi>\<^sub>T\<^sub>E \<Rightarrow> bool\<close> (\<open>_, _ \<Turnstile>\<^sub>T\<close> [50]) where
+fun semantics\<^sub>T :: \<open>trace \<Rightarrow> nat \<Rightarrow> \<Phi>\<^sub>T\<^sub>M \<Rightarrow> bool\<close> (\<open>_, _ \<Turnstile>\<^sub>T\<close> [50]) where
   \<open>s, i \<Turnstile>\<^sub>T \<bottom>\<^sub>T = False\<close> |
-  \<open>s, i \<Turnstile>\<^sub>T (Atom x) = ((\<Phi>\<^sub>P.Atom x)\<^bold>[s i\<^bold>]\<^sub>E)\<close> |
+  \<open>s, i \<Turnstile>\<^sub>T (Atom x) = ((\<Phi>\<^sub>P.Atom x)\<^bold>[s i\<^bold>]\<^sub>M)\<close> |
   \<open>s, i \<Turnstile>\<^sub>T (\<not>\<^sub>T p) = (\<not> (s, i \<Turnstile>\<^sub>T p))\<close> |
   \<open>s, i \<Turnstile>\<^sub>T (p \<longrightarrow>\<^sub>T q) = ((s, i \<Turnstile>\<^sub>T p) \<longrightarrow> (s, i \<Turnstile>\<^sub>T q))\<close> |
   \<open>s, i \<Turnstile>\<^sub>T (p \<or>\<^sub>T q) = ((s, i \<Turnstile>\<^sub>T p) \<or> (s, i \<Turnstile>\<^sub>T q))\<close> |
@@ -55,15 +59,15 @@ fun semantics\<^sub>T :: \<open>trace \<Rightarrow> nat \<Rightarrow> \<Phi>\<^s
   \<open>s, i \<Turnstile>\<^sub>T init = (i = 0)\<close> |
   \<open>s, i \<Turnstile>\<^sub>T (\<phi> until \<psi>) = ((\<exists> j \<ge> i. s, j \<Turnstile>\<^sub>T \<psi> \<and> (\<forall>k \<ge> i. j > k \<longrightarrow> s, k \<Turnstile>\<^sub>T \<phi>)) \<or> (\<forall>k \<ge> i. s, k \<Turnstile>\<^sub>T \<phi>))\<close>
 
-lemma sem\<^sub>T\<^sub>E_equiv: \<open>(\<forall>M. semantics\<^sub>E M p) \<longleftrightarrow> (\<forall>s i. (p\<^bold>[s i\<^bold>]\<^sub>E))\<close> 
+lemma sem\<^sub>T\<^sub>M_equiv: \<open>(\<forall>M. semantics\<^sub>M M p) \<longleftrightarrow> (\<forall>s i. (p\<^bold>[s i\<^bold>]\<^sub>M))\<close> 
   using st_nth.simps(1) by metis
 
-lemma sem\<^sub>T\<^sub>E_equiv2: \<open>s, i \<Turnstile>\<^sub>T (p\<^sup>T) \<longleftrightarrow> (p\<^bold>[s i\<^bold>]\<^sub>E)\<close> 
+lemma sem\<^sub>T\<^sub>M_equiv2: \<open>s, i \<Turnstile>\<^sub>T (p\<^sup>T) \<longleftrightarrow> (p\<^bold>[s i\<^bold>]\<^sub>M)\<close> 
   by (induct p) auto
 
-lemma \<open>(\<forall>M. semantics\<^sub>E M p) \<longleftrightarrow> (\<forall>s i. s, i \<Turnstile>\<^sub>T (p\<^sup>T))\<close> using sem\<^sub>T\<^sub>E_equiv sem\<^sub>T\<^sub>E_equiv2 by simp
+lemma \<open>(\<forall>M. semantics\<^sub>M M p) \<longleftrightarrow> (\<forall>s i. s, i \<Turnstile>\<^sub>T (p\<^sup>T))\<close> using sem\<^sub>T\<^sub>M_equiv sem\<^sub>T\<^sub>M_equiv2 by simp
 
-abbreviation semantics_trace\<^sub>T\<^sub>E :: \<open>trace set \<Rightarrow> \<Phi>\<^sub>T\<^sub>E \<Rightarrow> bool\<close> (infix \<open>\<Turnstile>\<^sub>T#\<close> 50) where
+abbreviation semantics_trace\<^sub>T\<^sub>M :: \<open>trace set \<Rightarrow> \<Phi>\<^sub>T\<^sub>M \<Rightarrow> bool\<close> (infix \<open>\<Turnstile>\<^sub>T#\<close> 50) where
   \<open>S \<Turnstile>\<^sub>T# \<phi> \<equiv> \<forall>s\<in>S. \<forall>i. (s, i \<Turnstile>\<^sub>T \<phi>)\<close>
 
 section \<open>Relations between Hoare Logic and Temporal Logic\<close>
@@ -71,10 +75,10 @@ section \<open>Relations between Hoare Logic and Temporal Logic\<close>
 subsection \<open>Unless\<close>
 
 \<comment> \<open>Theorem 4.15\<close>
-theorem unless_ht: \<open>(\<forall>b \<in> \<Pi>. (\<Turnstile>\<^sub>H \<^bold>{ \<phi> \<^bold>\<and> \<^bold>\<not> \<psi> \<^bold>} ((fst b) \<triangleright> do (snd b)) \<^bold>{ \<phi> \<^bold>\<or> \<psi> \<^bold>})) \<longleftrightarrow> Agent \<Turnstile>\<^sub>T# \<phi>\<^sup>E\<^sup>T unless \<psi>\<^sup>E\<^sup>T\<close>
+theorem unless_ht: \<open>(\<forall>b \<in> \<Pi>. (\<Turnstile>\<^sub>H \<^bold>{ \<phi> \<^bold>\<and> \<^bold>\<not> \<psi> \<^bold>} ((fst b) \<triangleright> do (snd b)) \<^bold>{ \<phi> \<^bold>\<or> \<psi> \<^bold>})) \<longleftrightarrow> Agent \<Turnstile>\<^sub>T# \<phi>\<^sup>T unless \<psi>\<^sup>T\<close>
 proof
   assume *: \<open>\<forall>b \<in> \<Pi>. (\<Turnstile>\<^sub>H \<^bold>{ \<phi> \<^bold>\<and> \<^bold>\<not> \<psi> \<^bold>} ((fst b) \<triangleright> do (snd b)) \<^bold>{ \<phi> \<^bold>\<or> \<psi> \<^bold>})\<close>
-  show \<open>Agent \<Turnstile>\<^sub>T# \<phi>\<^sup>E\<^sup>T unless \<psi>\<^sup>E\<^sup>T\<close> (is \<open>Agent \<Turnstile>\<^sub>T# ?\<phi> unless ?\<psi>\<close>)
+  show \<open>Agent \<Turnstile>\<^sub>T# \<phi>\<^sup>T unless \<psi>\<^sup>T\<close> (is \<open>Agent \<Turnstile>\<^sub>T# ?\<phi> unless ?\<psi>\<close>)
   proof (rule ccontr)
     assume \<open>\<not> Agent \<Turnstile>\<^sub>T# ?\<phi> unless ?\<psi>\<close>
     then obtain s i where \<open>\<not> (s, i \<Turnstile>\<^sub>T (?\<phi> unless ?\<psi>))\<close> \<open>s \<in> Agent\<close> by auto
@@ -91,10 +95,10 @@ proof
       moreover from this have \<open>k > i\<close> using \<open>s, i \<Turnstile>\<^sub>T ?\<phi>\<close> by fastforce
       ultimately have \<open>\<not> ?P (k - 1)\<close> by simp
       with \<open>k > i\<close> have \<open>s, k - 1 \<Turnstile>\<^sub>T (?\<phi> \<and>\<^sub>T \<not>\<^sub>T ?\<psi>)\<close> using a by simp
-      then have \<open>st_nth s (k - 1) \<Turnstile>\<^sub>M \<phi> \<^bold>\<and> \<^bold>\<not> \<psi>\<close> by (simp add: sem\<^sub>T\<^sub>E_equiv2 transfer_semantics\<^sub>M)
+      then have \<open>st_nth s (k - 1) \<Turnstile>\<^sub>M \<phi> \<^bold>\<and> \<^bold>\<not> \<psi>\<close> by (simp add: sem\<^sub>T\<^sub>M_equiv2 transfer_semantics\<^sub>M)
       moreover have \<open>?P k\<close> using Pk by simp
       then have \<open>s, k \<Turnstile>\<^sub>T (\<not>\<^sub>T ?\<phi> \<and>\<^sub>T \<not>\<^sub>T ?\<psi>)\<close> using a \<open>k > i\<close> by simp
-      then have \<open>st_nth s k \<Turnstile>\<^sub>M \<^bold>\<not> \<phi> \<^bold>\<and> \<^bold>\<not> \<psi>\<close> by (simp add: sem\<^sub>T\<^sub>E_equiv2 transfer_semantics\<^sub>M)
+      then have \<open>st_nth s k \<Turnstile>\<^sub>M \<^bold>\<not> \<phi> \<^bold>\<and> \<^bold>\<not> \<psi>\<close> by (simp add: sem\<^sub>T\<^sub>M_equiv2 transfer_semantics\<^sub>M)
       moreover obtain b where \<open>(fst b, snd b) = act_nth s (k - 1)\<close> by simp
       moreover from this have \<open>b \<in> \<Pi>\<close> using \<open>s \<in> Agent\<close> trace_in_\<Pi> unfolding Agent_def by simp
       with * have \<open>\<forall> s \<in> Agent. \<forall>i. ((\<phi> \<^bold>\<and> \<^bold>\<not> \<psi>)\<^bold>[s i\<^bold>]\<^sub>M) \<and> ((fst b) \<triangleright> do (snd b)) = (act_nth s i) \<longrightarrow> ((\<phi> \<^bold>\<or> \<psi>)\<^bold>[s (i+1)\<^bold>]\<^sub>M)\<close>
@@ -132,7 +136,7 @@ proof
         with \<open>\<not> s, i \<Turnstile>\<^sub>T (?\<phi> until ?\<psi>)\<close> show ?thesis by fastforce
       qed simp
       ultimately have \<open>s, j - 1 \<Turnstile>\<^sub>T (?\<phi> \<and>\<^sub>T \<not>\<^sub>T ?\<psi>)\<close> by simp
-      then have \<open>st_nth s (j - 1) \<Turnstile>\<^sub>M \<phi> \<^bold>\<and> \<^bold>\<not> \<psi>\<close> by (simp add: sem\<^sub>T\<^sub>E_equiv2 transfer_semantics\<^sub>M)
+      then have \<open>st_nth s (j - 1) \<Turnstile>\<^sub>M \<phi> \<^bold>\<and> \<^bold>\<not> \<psi>\<close> by (simp add: sem\<^sub>T\<^sub>M_equiv2 transfer_semantics\<^sub>M)
       moreover 
       {
         have \<open>\<not> s, j \<Turnstile>\<^sub>T ?\<phi>\<close> using Pj by simp
@@ -140,7 +144,7 @@ proof
         then have \<open>\<not> ?P j\<close> using Pk by simp
         then have \<open>\<not> s, j \<Turnstile>\<^sub>T ?\<psi>\<close> using Pj by simp
         ultimately have \<open>s, j \<Turnstile>\<^sub>T (\<not>\<^sub>T ?\<phi> \<and>\<^sub>T \<not>\<^sub>T ?\<psi>)\<close> by simp
-        then have \<open>st_nth s j \<Turnstile>\<^sub>M \<^bold>\<not> \<phi> \<^bold>\<and> \<^bold>\<not> \<psi>\<close> by (simp add: sem\<^sub>T\<^sub>E_equiv2 transfer_semantics\<^sub>M)
+        then have \<open>st_nth s j \<Turnstile>\<^sub>M \<^bold>\<not> \<phi> \<^bold>\<and> \<^bold>\<not> \<psi>\<close> by (simp add: sem\<^sub>T\<^sub>M_equiv2 transfer_semantics\<^sub>M)
       }
       moreover obtain b where \<open>(fst b, snd b) = act_nth s (j - 1)\<close> by simp
       moreover from this have \<open>b \<in> \<Pi>\<close> using \<open>s \<in> Agent\<close> trace_in_\<Pi> unfolding Agent_def by simp
@@ -154,7 +158,7 @@ proof
     qed
   qed
 next
-  assume \<open>Agent \<Turnstile>\<^sub>T# \<phi>\<^sup>E\<^sup>T unless \<psi>\<^sup>E\<^sup>T\<close> (is \<open>Agent \<Turnstile>\<^sub>T# ?\<phi> unless ?\<psi>\<close>)
+  assume \<open>Agent \<Turnstile>\<^sub>T# \<phi>\<^sup>T unless \<psi>\<^sup>T\<close> (is \<open>Agent \<Turnstile>\<^sub>T# ?\<phi> unless ?\<psi>\<close>)
   show \<open>\<forall>b \<in> \<Pi>. (\<Turnstile>\<^sub>H \<^bold>{ \<phi> \<^bold>\<and> \<^bold>\<not> \<psi> \<^bold>} ((fst b) \<triangleright> do (snd b)) \<^bold>{ \<phi> \<^bold>\<or> \<psi> \<^bold>})\<close>
   proof 
     fix b
@@ -171,7 +175,7 @@ next
           show \<open>((\<phi> \<^bold>\<and> \<^bold>\<not> \<psi>)\<^bold>[s i\<^bold>]\<^sub>M) \<and> ((fst b) \<triangleright> do (snd b)) = (act_nth s i) \<longrightarrow> ((\<phi> \<^bold>\<or> \<psi>)\<^bold>[s (i+1)\<^bold>]\<^sub>M)\<close>
           proof (cases \<open>st_nth s i \<Turnstile>\<^sub>M \<phi>\<close>)
             case True
-            then have \<open>s, i \<Turnstile>\<^sub>T ?\<phi>\<close> by (simp add: sem\<^sub>T\<^sub>E_equiv2 transfer_semantics\<^sub>M)
+            then have \<open>s, i \<Turnstile>\<^sub>T ?\<phi>\<close> by (simp add: sem\<^sub>T\<^sub>M_equiv2 transfer_semantics\<^sub>M)
             with \<open>Agent \<Turnstile>\<^sub>T# ?\<phi> unless ?\<psi>\<close> have \<open>s, i \<Turnstile>\<^sub>T (?\<phi> until ?\<psi>)\<close> using \<open>s \<in> Agent\<close> unfolding unless_def by simp
             then have \<open>(\<exists> j \<ge> i. (s, j \<Turnstile>\<^sub>T ?\<psi>) \<and> (\<forall>k \<ge> i. j > k \<longrightarrow> (s, k \<Turnstile>\<^sub>T ?\<phi>))) \<or> (\<forall>k \<ge> i. (s, k \<Turnstile>\<^sub>T ?\<phi>))\<close> by simp
             then obtain j where *: \<open>(j \<ge> i \<and> s, j \<Turnstile>\<^sub>T ?\<psi> \<and> (\<forall>k \<ge> i. j > k \<longrightarrow> s, k \<Turnstile>\<^sub>T ?\<phi>)) \<or> s, i + 1 \<Turnstile>\<^sub>T ?\<phi>\<close> by auto
@@ -179,7 +183,7 @@ next
             proof (cases \<open>j > i + 1\<close>)
               case True
               with * have \<open>s, (i + 1) \<Turnstile>\<^sub>T ?\<phi>\<close> by auto
-              then have \<open>st_nth s (i + 1) \<Turnstile>\<^sub>M \<phi> \<^bold>\<or> \<psi>\<close> by (simp add: sem\<^sub>T\<^sub>E_equiv2 transfer_semantics\<^sub>M)
+              then have \<open>st_nth s (i + 1) \<Turnstile>\<^sub>M \<phi> \<^bold>\<or> \<psi>\<close> by (simp add: sem\<^sub>T\<^sub>M_equiv2 transfer_semantics\<^sub>M)
               then show ?thesis by simp
             next
               case False
@@ -188,9 +192,9 @@ next
               then show ?thesis
               proof (cases \<open>st_nth s i \<Turnstile>\<^sub>M \<psi>\<close>)
                 case False
-                then have \<open>\<not> s, i \<Turnstile>\<^sub>T ?\<psi>\<close> by (simp add: sem\<^sub>T\<^sub>E_equiv2 transfer_semantics\<^sub>M)
+                then have \<open>\<not> s, i \<Turnstile>\<^sub>T ?\<psi>\<close> by (simp add: sem\<^sub>T\<^sub>M_equiv2 transfer_semantics\<^sub>M)
                 with ** have \<open>s, i + 1 \<Turnstile>\<^sub>T ?\<psi> \<or> s, i + 1 \<Turnstile>\<^sub>T ?\<phi>\<close> by simp
-                then show ?thesis using sem\<^sub>T\<^sub>E_equiv2 transfer_semantics\<^sub>M by auto
+                then show ?thesis using sem\<^sub>T\<^sub>M_equiv2 transfer_semantics\<^sub>M by auto
               qed simp
             qed
           qed simp
@@ -210,7 +214,7 @@ definition ensures :: \<open>'a \<Phi>\<^sub>T \<Rightarrow> 'a \<Phi>\<^sub>T \
 theorem ex_ensures:
   assumes \<open>\<forall>b \<in> \<Pi>. (\<Turnstile>\<^sub>H \<^bold>{ \<phi> \<^bold>\<and> \<^bold>\<not> \<psi> \<^bold>} ((fst b) \<triangleright> do (snd b)) \<^bold>{ \<phi> \<^bold>\<or> \<psi> \<^bold>})\<close> 
       and \<open>\<exists>b \<in> \<Pi>. (\<Turnstile>\<^sub>H \<^bold>{ \<phi> \<^bold>\<and> \<^bold>\<not> \<psi> \<^bold>} ((fst b) \<triangleright> do (snd b)) \<^bold>{ \<psi> \<^bold>})\<close>
-    shows \<open>Agent \<Turnstile>\<^sub>T# \<phi>\<^sup>E\<^sup>T ensures \<psi>\<^sup>E\<^sup>T\<close> (is \<open>Agent \<Turnstile>\<^sub>T# ?\<phi> ensures ?\<psi>\<close>)
+    shows \<open>Agent \<Turnstile>\<^sub>T# \<phi>\<^sup>T ensures \<psi>\<^sup>T\<close> (is \<open>Agent \<Turnstile>\<^sub>T# ?\<phi> ensures ?\<psi>\<close>)
 proof
   fix s
   assume \<open>s \<in> Agent\<close>
@@ -238,10 +242,10 @@ proof
             using \<open>fair_trace s\<close> unfolding fair_trace_def by fastforce
           ultimately have \<open>\<exists>j > i. ((\<phi> \<^bold>\<and> \<^bold>\<not> \<psi>)\<^bold>[s j\<^bold>]\<^sub>M) \<longrightarrow> (\<psi>\<^bold>[s (j+1)\<^bold>]\<^sub>M)\<close> by auto
           moreover from \<open>\<forall>j > i. s, j \<Turnstile>\<^sub>T (?\<phi> \<and>\<^sub>T \<not>\<^sub>T ?\<psi>)\<close> have \<open>\<forall>j > i. ((\<phi> \<^bold>\<and> \<^bold>\<not> \<psi>)\<^bold>[s j\<^bold>]\<^sub>M)\<close> 
-            using sem\<^sub>T\<^sub>E_equiv2 transfer_semantics\<^sub>M by simp
+            using sem\<^sub>T\<^sub>M_equiv2 transfer_semantics\<^sub>M by simp
           ultimately have \<open>\<exists>j > i. (\<psi>\<^bold>[s (j+1)\<^bold>]\<^sub>M)\<close> by auto
         }
-      ultimately show False using sem\<^sub>T\<^sub>E_equiv2 transfer_semantics\<^sub>M by auto
+      ultimately show False using sem\<^sub>T\<^sub>M_equiv2 transfer_semantics\<^sub>M by auto
       qed
     qed
     ultimately show \<open>s, i \<Turnstile>\<^sub>T (?\<phi> ensures ?\<psi>)\<close> by (simp add: ensures_def)
@@ -254,26 +258,38 @@ fun disL:: \<open>'a \<Phi>\<^sub>T list \<Rightarrow> 'a \<Phi>\<^sub>T\<close>
   \<open>disL [] = \<bottom>\<^sub>T\<close> |
   \<open>disL (\<phi> # \<phi>\<^sub>L) = \<phi> \<or>\<^sub>T disL \<phi>\<^sub>L\<close>
 
-inductive leads_to :: \<open>\<Phi>\<^sub>T\<^sub>E \<Rightarrow> \<Phi>\<^sub>T\<^sub>E \<Rightarrow> bool\<close> (infix \<open>\<mapsto>\<close> 55) where
-  ensures: \<open>\<forall>s i. s, i \<Turnstile>\<^sub>T (\<phi> ensures \<psi>) \<Longrightarrow> \<phi> \<mapsto> \<psi>\<close> |
+inductive leads_to :: \<open>\<Phi>\<^sub>T\<^sub>M \<Rightarrow> \<Phi>\<^sub>T\<^sub>M \<Rightarrow> bool\<close> (infix \<open>\<mapsto>\<close> 55) where
+  ensures: \<open>\<forall>s \<in> Agent. \<forall>i. s, i \<Turnstile>\<^sub>T (\<phi> ensures \<psi>) \<Longrightarrow> \<phi> \<mapsto> \<psi>\<close> |
   imp: \<open>\<phi> \<mapsto> \<chi> \<Longrightarrow> \<chi> \<mapsto> \<psi> \<Longrightarrow> \<phi> \<mapsto> \<psi>\<close> |
   disj: \<open>\<forall>\<phi> \<in> set \<phi>\<^sub>L. \<phi> \<mapsto> \<psi> \<Longrightarrow> disL \<phi>\<^sub>L \<mapsto> \<psi>\<close>
 
 \<comment> \<open>Lemma 4.18\<close>
-lemma \<open>\<phi> \<mapsto> \<psi> \<Longrightarrow> s, i \<Turnstile>\<^sub>T (\<phi> \<longrightarrow>\<^sub>T \<diamondop>\<psi>)\<close>
-proof (induct arbitrary: i rule: leads_to.inducts)
+lemma leads_to_temp: \<open>\<phi> \<mapsto> \<psi> \<Longrightarrow> \<forall>s \<in> Agent. \<forall>i. s, i \<Turnstile>\<^sub>T (\<phi> \<longrightarrow>\<^sub>T \<diamondop>\<psi>)\<close>
+proof (induct rule: leads_to.inducts)
   case (ensures \<phi> \<psi>)
   then show ?case unfolding ensures_def always_def eventuality_def by simp
 next
   case (imp \<phi> \<chi> \<psi>)
-  then have \<open>s, i \<Turnstile>\<^sub>T \<phi> \<longrightarrow> s, i \<Turnstile>\<^sub>T (\<diamondop> \<chi>)\<close> by simp
-  moreover have \<open>s, i \<Turnstile>\<^sub>T (\<diamondop> \<chi>) \<longrightarrow> (\<exists>j \<ge> i. s, j \<Turnstile>\<^sub>T \<chi>)\<close> 
-    unfolding eventuality_def always_def by simp
-  then have \<open>s, i \<Turnstile>\<^sub>T (\<diamondop> \<chi>) \<longrightarrow> (\<exists>j \<ge> i. s, j \<Turnstile>\<^sub>T \<psi>)\<close> using imp(4) unfolding eventuality_def always_def
-    using order_trans by fastforce
-  then have \<open>s, i \<Turnstile>\<^sub>T (\<diamondop> \<chi>) \<longrightarrow> s, i \<Turnstile>\<^sub>T (\<diamondop> \<psi>)\<close> by (simp add: eventuality_def always_def)
-  ultimately have \<open>s, i \<Turnstile>\<^sub>T \<phi> \<longrightarrow> s, i \<Turnstile>\<^sub>T (\<diamondop> \<psi>)\<close> by simp
-  then show ?case by simp
+  show ?case
+  proof
+    fix s
+    assume \<open>s \<in> Agent\<close>
+    show \<open>\<forall>i. s, i \<Turnstile>\<^sub>T (\<phi> \<longrightarrow>\<^sub>T \<diamondop>\<psi>)\<close>
+    proof
+      fix i
+      have \<open>s, i \<Turnstile>\<^sub>T \<phi> \<longrightarrow> s, i \<Turnstile>\<^sub>T (\<diamondop> \<psi>)\<close> 
+      proof
+        assume \<open>s, i \<Turnstile>\<^sub>T \<phi>\<close>
+        with \<open>s \<in> Agent\<close> have \<open>s, i \<Turnstile>\<^sub>T (\<diamondop> \<chi>)\<close> using imp(2) by simp
+        then obtain j where \<open>j \<ge> i\<close> \<open>s, j \<Turnstile>\<^sub>T \<chi>\<close> unfolding eventuality_def always_def by auto
+        with \<open>s \<in> Agent\<close> have \<open>s, j \<Turnstile>\<^sub>T (\<diamondop> \<psi>)\<close> using imp(4) by simp
+        then obtain k where \<open>k \<ge> j\<close> \<open>s, k \<Turnstile>\<^sub>T \<psi>\<close> unfolding eventuality_def always_def by auto
+        with \<open>j \<ge> i\<close> show \<open>s, i \<Turnstile>\<^sub>T (\<diamondop> \<psi>)\<close> 
+          using order.trans unfolding eventuality_def always_def by auto
+      qed
+      then show \<open>s, i \<Turnstile>\<^sub>T (\<phi> \<longrightarrow>\<^sub>T \<diamondop> \<psi>)\<close> by simp
+    qed
+  qed
 next
   case (disj \<phi>\<^sub>L \<psi>)
   then show ?case by (induct \<phi>\<^sub>L) simp_all
