Gvf_Example_BW4T.thy
@@ -1,91 +1,179 @@
-theory Gvf_Example_BW4T imports Gvf_Agent_Specification begin
+theory Gvf_Example_BW4T imports Gvf_Temporal_Logic begin
 
 section \<open>Example BW4T single agent specification.\<close>
 
-\<comment> \<open>Proof of concept. Only part of the specification is included so far and proofs are missing.
-   Mainly due to the temporal logic layer still missing.\<close>
+subsection \<open>Agent specification setup\<close>
 
-\<comment> \<open>Set up agent specification-\<close>
-\<comment> \<open>Propositions:\<close>
-abbreviation \<open>in_dropzone::\<Phi>\<^sub>L \<equiv> Atom 0\<close>
-abbreviation \<open>in_room::\<Phi>\<^sub>L \<equiv> Atom 1\<close>
-abbreviation \<open>collect_red::\<Phi>\<^sub>L \<equiv> Atom 2\<close>
+\<comment> \<open>Propositions.\<close>
+abbreviation \<open>in_dropzone::\<Phi>\<^sub>L \<equiv> \<Phi>\<^sub>P.Atom 0\<close>
+abbreviation \<open>in_r\<^sub>1::\<Phi>\<^sub>L \<equiv> \<Phi>\<^sub>P.Atom 1\<close>
+abbreviation \<open>collect_red::\<Phi>\<^sub>L \<equiv> \<Phi>\<^sub>P.Atom 2\<close>
+abbreviation \<open>holding_b\<^sub>1::\<Phi>\<^sub>L \<equiv> \<Phi>\<^sub>P.Atom 3\<close>
+abbreviation \<open>atBlock_b\<^sub>1::\<Phi>\<^sub>L \<equiv> \<Phi>\<^sub>P.Atom 4\<close>
 
-\<comment> \<open>Actions:\<close>
-abbreviation \<open>goto_dropzone_Bcap \<equiv> 0::nat\<close>
-abbreviation \<open>goto_dropzone \<equiv> basic goto_dropzone_Bcap\<close>
+\<comment> \<open>Actions.\<close>
+abbreviation \<open>goTo_dropzone \<equiv> basic 0\<close>
+abbreviation \<open>goTo_r\<^sub>1::cap \<equiv> basic 1\<close>
+abbreviation \<open>goToBlock_b\<^sub>1::cap \<equiv> basic 2\<close>
+abbreviation \<open>pickUp_b\<^sub>1::cap \<equiv> basic 3\<close>
+abbreviation \<open>putDown::cap \<equiv> basic 4\<close>
 
-abbreviation \<open>goto_room_Bcap \<equiv> 1::nat\<close>
-abbreviation \<open>goto_room::cap \<equiv> basic goto_room_Bcap\<close>
+\<comment> \<open>Specification of the program.\<close>
+abbreviation 
+  \<open>\<Pi>\<^sub>x \<equiv> [ 
+    (B in_r\<^sub>1 \<^bold>\<and> B holding_b\<^sub>1) \<triangleright> do goTo_dropzone,
+    (B (\<^bold>\<not> in_r\<^sub>1) \<^bold>\<and> B (\<^bold>\<not> holding_b\<^sub>1) ) \<triangleright> do goTo_r\<^sub>1,
+    (B in_r\<^sub>1 \<^bold>\<and> B (\<^bold>\<not> holding_b\<^sub>1) \<^bold>\<and> B (\<^bold>\<not> atBlock_b\<^sub>1)) \<triangleright> do goToBlock_b\<^sub>1,
+    (B atBlock_b\<^sub>1 \<^bold>\<and> B (\<^bold>\<not> holding_b\<^sub>1)) \<triangleright> do pickUp_b\<^sub>1,
+    (B holding_b\<^sub>1 \<^bold>\<and> B in_dropzone) \<triangleright> do putDown
+  ]\<close>
 
-\<comment> \<open>Specification of the program:\<close>
-abbreviation \<open>\<Pi>\<^sub>x \<equiv> { (B in_dropzone) \<triangleright> do goto_room }\<close>
-abbreviation \<open>M\<^sub>0\<^sub>x \<equiv> ( { in_dropzone }, { collect_red } )\<close>
-abbreviation \<open>S\<^sub>x \<equiv> [(goto_room_Bcap, \<top>\<^sub>M, [\<^bold>{ B in_dropzone \<^bold>} goto_room \<^bold>{ B in_room \<^bold>}])]\<close>
+abbreviation 
+  \<open>M\<^sub>0\<^sub>x \<equiv> ( { in_dropzone, \<^bold>\<not> in_r\<^sub>1, \<^bold>\<not> holding_b\<^sub>1, \<^bold>\<not> atBlock_b\<^sub>1 }, { collect_red } )\<close>
+
+abbreviation 
+  \<open>S\<^sub>x' \<equiv> [
+    (0, fst (\<Pi>\<^sub>x!0), 
+      [
+        \<^bold>{ B in_r\<^sub>1 \<^bold>\<and> B (\<^bold>\<not> in_dropzone) \<^bold>\<and> B holding_b\<^sub>1 \<^bold>} goTo_dropzone \<^bold>{ B (\<^bold>\<not> in_r\<^sub>1) \<^bold>\<and> B in_dropzone \<^bold>}
+      ]),
+
+    (1, fst (\<Pi>\<^sub>x!1), 
+      [
+        \<^bold>{ B (\<^bold>\<not> in_r\<^sub>1) \<^bold>\<and> B in_dropzone \<^bold>\<and> B (\<^bold>\<not> holding_b\<^sub>1) \<^bold>} goTo_r\<^sub>1 \<^bold>{ B in_r\<^sub>1 \<^bold>\<and> B (\<^bold>\<not> in_dropzone) \<^bold>}
+      ]),
+
+    (2, fst (\<Pi>\<^sub>x!2), 
+      [
+        \<^bold>{ B in_r\<^sub>1 \<^bold>\<and> B (\<^bold>\<not> atBlock_b\<^sub>1) \<^bold>\<and> B (\<^bold>\<not> holding_b\<^sub>1) \<^bold>} goToBlock_b\<^sub>1 \<^bold>{ B atBlock_b\<^sub>1 \<^bold>}
+      ]),
+
+    (3, fst (\<Pi>\<^sub>x!3), 
+      [
+        \<^bold>{ B atBlock_b\<^sub>1 \<^bold>\<and> B (\<^bold>\<not> holding_b\<^sub>1) \<^bold>} pickUp_b\<^sub>1 \<^bold>{ B holding_b\<^sub>1 \<^bold>}
+      ]),
+
+    (4, fst (\<Pi>\<^sub>x!4), 
+      [
+        \<^bold>{ B in_dropzone \<^bold>\<and> B holding_b\<^sub>1 \<^bold>} putDown \<^bold>{ B collect_red \<^bold>}
+      ])
+  ]\<close>
+
+
+abbreviation 
+  \<open>inv\<^sub>x \<equiv> [
+    B in_dropzone \<^bold>\<longrightarrow> B (\<^bold>\<not> in_r\<^sub>1),
+    B in_r\<^sub>1 \<^bold>\<longrightarrow> B (\<^bold>\<not> in_dropzone)
+  ]\<close>
+
+abbreviation
+  \<open>S\<^sub>x \<equiv> add_invariants S\<^sub>x' inv\<^sub>x\<close>
 
 \<comment> \<open>Prove that the example is an instance of the single agent program locale.\<close>
 \<comment> \<open>We use a trick where \<T> is simply some function that complies to our definition due to Hilbert's epsilon operator i.e. the axiom of choice.\<close>
-interpretation example: single_agent_program \<open>SOME \<T>. complies S\<^sub>x \<T>\<close> \<Pi>\<^sub>x M\<^sub>0\<^sub>x S\<^sub>x
+global_interpretation bw4t: single_agent_program \<open>SOME \<T>. complies S\<^sub>x \<T>\<close> \<open>set \<Pi>\<^sub>x\<close> M\<^sub>0\<^sub>x S\<^sub>x
+  defines semantics\<^sub>H (\<open>\<Turnstile>\<^sub>H\<close>) = bw4t.semantics\<^sub>H
+      and derive\<^sub>H (\<open>\<turnstile>\<^sub>H\<close>) = bw4t.derive\<^sub>H
+      and leads_to (infix \<open>\<mapsto>\<close> 55) = bw4t.leads_to
 proof -
   let ?\<T> = \<open>SOME \<T>. complies S\<^sub>x \<T>\<close>
-  (* This could be harder to proof than suggested since S\<^sub>x here has one element *)
-  have satisfiable: \<open>satisfiable S\<^sub>x\<close> unfolding satisfiable_def 
-  proof 
-    fix M
-    let ?n = \<open>goto_room_Bcap\<close> and ?\<Phi> = \<open>\<top>\<^sub>M\<close> and ?hts = \<open>[\<^bold>{ B in_dropzone \<^bold>} goto_room \<^bold>{ B in_room \<^bold>}]\<close>
-    let ?sat_hts = \<open>{ht \<in> set ?hts. M \<Turnstile>\<^sub>M pre ht }\<close>
-    have \<open>\<exists>M'. M' \<Turnstile>\<^sub>M (B in_room) \<and> \<not> fst M' \<Turnstile>\<^sub>L \<bottom>\<^sub>L\<close> 
-    proof -
-      have \<open>({in_room}, {}) \<Turnstile>\<^sub>M B in_room\<close> by simp
-      moreover have \<open>\<not> fst ({in_room}, {}) \<Turnstile>\<^sub>L \<bottom>\<^sub>L\<close> by auto
-      ultimately show ?thesis by blast
-    qed
-    then have \<open>(M \<Turnstile>\<^sub>M ?\<Phi> \<longrightarrow> (\<exists>\<Sigma>'. (\<not> fst M \<Turnstile>\<^sub>L \<bottom>\<^sub>L \<longrightarrow> \<not> \<Sigma>' \<Turnstile>\<^sub>L \<bottom>\<^sub>L) \<and> (let \<Gamma>' = snd M - {\<psi> \<in> snd M. \<Sigma>' \<Turnstile>\<^sub>L \<psi>} in (\<forall>ht \<in> ?sat_hts. (\<Sigma>', \<Gamma>') \<Turnstile>\<^sub>M post ht)))) \<and> (M \<Turnstile>\<^sub>M \<^bold>\<not> ?\<Phi> \<longrightarrow> (\<forall>ht\<in>?sat_hts. M \<Turnstile>\<^sub>M post ht))\<close> by auto
-    then show 
-      \<open>\<forall>s\<in>set S\<^sub>x. let (_, \<Phi>, hts) = s; sat_hts = {ht \<in> set hts. M \<Turnstile>\<^sub>M pre ht} in 
-        (M \<Turnstile>\<^sub>M \<Phi> \<longrightarrow> (\<exists>M'. (\<not> fst M \<Turnstile>\<^sub>L \<bottom>\<^sub>L \<longrightarrow> \<not> fst M' \<Turnstile>\<^sub>L \<bottom>\<^sub>L) \<and> (snd M' = snd M - {\<psi> \<in> snd M. fst M' \<Turnstile>\<^sub>L \<psi>}) \<and> (\<forall>ht \<in> sat_hts. M' \<Turnstile>\<^sub>M post ht))) \<and> 
-        (M \<Turnstile>\<^sub>M \<^bold>\<not> \<Phi> \<longrightarrow> (\<forall>ht\<in>sat_hts. M \<Turnstile>\<^sub>M post ht))\<close>
-      by simp
-  qed
-  then have s: \<open>is_ht_specification S\<^sub>x\<close> unfolding is_ht_specification_def by simp
-  then have c: \<open>complies S\<^sub>x ?\<T>\<close> using model_exists by (simp add: someI2_ex)
-  show \<open>single_agent_program ?\<T> \<Pi>\<^sub>x M\<^sub>0\<^sub>x S\<^sub>x\<close>
+  have \<open>\<nabla> M\<^sub>0\<^sub>x\<close> unfolding is_mental_state_def by fastforce
+  moreover have \<open>satisfiable S\<^sub>x\<close> unfolding satisfiable_def
   proof
-    have \<open>\<nabla> M\<^sub>0\<^sub>x\<close>
-    proof - 
-      have \<open>\<not> {in_dropzone} \<Turnstile>\<^sub>L \<bottom>\<^sub>L\<close> by auto
-      moreover have \<open>in_dropzone \<noteq> collect_red\<close> by simp
-      with neq_atom_not_entail have \<open>\<not> {in_dropzone} \<Turnstile>\<^sub>L collect_red\<close> by metis
-      moreover have \<open>\<not> {} \<Turnstile>\<^sub>L \<^bold>\<not> in_dropzone\<close> by auto
-      ultimately show ?thesis unfolding is_mental_state_def by auto
-    qed
-    then show \<open>\<Pi>\<^sub>x \<noteq> {} \<and> \<nabla> M\<^sub>0\<^sub>x\<close> by simp
-  next
-    fix \<Sigma> \<Gamma> n
-    show \<open>(\<exists>\<phi>. (\<phi>, basic n) \<in> \<Pi>\<^sub>x) \<longrightarrow> \<not> \<Sigma> \<Turnstile>\<^sub>L \<bottom>\<^sub>L \<longrightarrow> ?\<T> n (\<Sigma>, \<Gamma>) \<noteq> None \<longrightarrow> \<not> the (?\<T> n (\<Sigma>, \<Gamma>)) \<Turnstile>\<^sub>L \<bottom>\<^sub>L\<close> 
-    proof
-      assume \<open>\<exists>\<phi>. (\<phi>, basic n) \<in> \<Pi>\<^sub>x\<close>
-      from c have \<open>\<forall>s\<in>set S\<^sub>x. complies_hts s ?\<T>\<close> unfolding complies_def by simp
-      then have \<open>\<forall>s\<in>set S\<^sub>x. \<forall>ht\<in>set (snd (snd s)). complies_ht (\<Sigma>, \<Gamma>) ?\<T> (fst (snd s)) (the (htb_basic_unpack ht))\<close> unfolding complies_hts_def by blast
-      moreover have \<open>\<forall>s\<in>set S\<^sub>x. \<forall>ht\<in>set (snd (snd s)). fst s = (fst (snd ((the (htb_basic_unpack ht)))))\<close> by simp
-      ultimately have \<open>\<forall>s\<in>set S\<^sub>x. \<forall>ht\<in>set (snd (snd s)). \<not> \<Sigma> \<Turnstile>\<^sub>L \<bottom>\<^sub>L \<longrightarrow> ?\<T> (fst s) (\<Sigma>, \<Gamma>) \<noteq> None \<longrightarrow> \<not>the (?\<T> (fst s) (\<Sigma>, \<Gamma>)) \<Turnstile>\<^sub>L \<bottom>\<^sub>L\<close> by simp
-      then have \<open>\<forall>s\<in>set S\<^sub>x. \<not> \<Sigma> \<Turnstile>\<^sub>L \<bottom>\<^sub>L \<longrightarrow> ?\<T> (fst s) (\<Sigma>, \<Gamma>) \<noteq> None \<longrightarrow> \<not>the (?\<T> (fst s) (\<Sigma>, \<Gamma>)) \<Turnstile>\<^sub>L \<bottom>\<^sub>L\<close> by simp
-      with \<open>\<exists>\<phi>. (\<phi>, basic n) \<in> \<Pi>\<^sub>x\<close> show \<open>\<not> \<Sigma> \<Turnstile>\<^sub>L \<bottom>\<^sub>L \<longrightarrow> ?\<T> n (\<Sigma>, \<Gamma>) \<noteq> None \<longrightarrow> \<not> the (?\<T> n (\<Sigma>, \<Gamma>)) \<Turnstile>\<^sub>L \<bottom>\<^sub>L\<close> by simp
-    qed
-  next
-    fix n M
-    have *: \<open>n \<notin> set (map fst S\<^sub>x) \<longrightarrow> (\<forall>M. ?\<T> n M = None)\<close> using c unfolding complies_def by simp
-    then have \<open>n \<notin> set (map fst S\<^sub>x) \<longrightarrow> ?\<T> n M = None\<close> by blast
-    show \<open>?\<T> n M \<noteq> None \<longrightarrow> (\<exists>\<phi>. (\<phi>, basic n) \<in> \<Pi>\<^sub>x)\<close>
-    proof
-      assume \<open>?\<T> n M \<noteq> None\<close>
-      then have \<open>n \<in> set (map fst S\<^sub>x)\<close> using * by metis
-      then show \<open>\<exists>\<phi>. (\<phi>, basic n) \<in> \<Pi>\<^sub>x\<close> by simp
-    qed
-  next
-    show \<open>is_ht_specification S\<^sub>x\<close> using s .
-    show \<open>complies S\<^sub>x ?\<T>\<close> using c .
+    fix M
+    let ?sat = \<open>\<lambda>s \<Sigma>. (M \<Turnstile>\<^sub>M fst (snd s) \<longrightarrow> satisfiable_base M (snd (snd s)) \<Sigma>) \<and> (M \<Turnstile>\<^sub>M \<^bold>\<not> (fst (snd s)) \<longrightarrow> (\<forall>ht \<in> set (snd (snd s)). M \<Turnstile>\<^sub>M pre ht \<longrightarrow> M \<Turnstile>\<^sub>M post ht))\<close>
+    \<comment> \<open>0\<close>
+    have \<open>?sat (S\<^sub>x!0) {\<^bold>\<not> in_r\<^sub>1 \<^bold>\<and> in_dropzone}\<close>
+      unfolding satisfiable_base_def using bel_dist_conj by auto
+    then have \<open>satisfiable_elem M (S\<^sub>x!0)\<close> using satisfiable_elem_def by auto
+    \<comment> \<open>1\<close>
+    moreover have \<open>?sat (S\<^sub>x!1) {in_r\<^sub>1 \<^bold>\<and> \<^bold>\<not> in_dropzone}\<close>
+      unfolding satisfiable_base_def using bel_dist_conj by auto
+    then have \<open>satisfiable_elem M (S\<^sub>x!1)\<close> using satisfiable_elem_def by auto
+    \<comment> \<open>2\<close>
+    moreover have \<open>?sat (S\<^sub>x!2) {atBlock_b\<^sub>1}\<close>
+      unfolding satisfiable_base_def using bel_dist_conj by auto
+    then have \<open>satisfiable_elem M (S\<^sub>x!2)\<close> using satisfiable_elem_def by auto
+    \<comment> \<open>3\<close>
+    moreover have \<open>?sat (S\<^sub>x!3) {holding_b\<^sub>1}\<close> 
+      unfolding satisfiable_base_def using bel_dist_conj by auto
+    then have \<open>satisfiable_elem M (S\<^sub>x!3)\<close> using satisfiable_elem_def by auto
+    \<comment> \<open>4\<close>
+    moreover have \<open>?sat (S\<^sub>x!4) {collect_red}\<close> 
+      unfolding satisfiable_base_def using bel_dist_conj by auto
+    then have \<open>satisfiable_elem M (S\<^sub>x!4)\<close> using satisfiable_elem_def by auto
+    \<comment> \<open>Combine\<close>
+    ultimately show \<open>\<forall>s\<in>set S\<^sub>x. satisfiable_elem M s\<close> by simp
   qed
+  then have \<open>is_ht_specification S\<^sub>x\<close> unfolding is_ht_specification_def by simp
+  moreover have \<open>\<forall>a. (\<exists>\<phi>. (\<phi>, basic a) \<in> set \<Pi>\<^sub>x) = (a \<in> set (map fst S\<^sub>x))\<close> by fastforce
+  ultimately show \<open>single_agent_program ?\<T> (set \<Pi>\<^sub>x) M\<^sub>0\<^sub>x S\<^sub>x\<close> using is_ht_spec_single_agent_program by simp
 qed
+
+subsection \<open>Correctness proof\<close>
+
+abbreviation \<open>M\<^sub>0 \<equiv> B in_dropzone \<^bold>\<and> G collect_red\<close>
+abbreviation \<open>M\<^sub>1 \<equiv> B in_r\<^sub>1 \<^bold>\<and> G collect_red\<close>
+abbreviation \<open>M\<^sub>2 \<equiv> B in_r\<^sub>1 \<^bold>\<and> B atBlock_b\<^sub>1 \<^bold>\<and> G collect_red\<close>
+abbreviation \<open>M\<^sub>3 \<equiv> B in_r\<^sub>1 \<^bold>\<and> B holding_b\<^sub>1 \<^bold>\<and> G collect_red\<close>
+abbreviation \<open>M\<^sub>4 \<equiv> B in_dropzone \<^bold>\<and> B holding_b\<^sub>1 \<^bold>\<and> G collect_red\<close>
+abbreviation \<open>M\<^sub>5 \<equiv> B collect_red\<close>
+
+lemma bw4t_lt: \<open>M\<^sub>0\<^sup>T \<mapsto> M\<^sub>5\<^sup>T\<close>
+proof -
+  have \<open>M\<^sub>0\<^sup>T \<mapsto> M\<^sub>1\<^sup>T\<close>
+  proof -
+    have \<open>\<forall>b \<in> set \<Pi>\<^sub>x. \<Turnstile>\<^sub>H \<^bold>{ M\<^sub>0 \<^bold>\<and> \<^bold>\<not> M\<^sub>1 \<^bold>} ((fst b) \<triangleright> do (snd b)) \<^bold>{ M\<^sub>0 \<^bold>\<or> M\<^sub>1 \<^bold>}\<close> sorry
+    moreover have \<open>\<exists>b \<in> set \<Pi>\<^sub>x. \<Turnstile>\<^sub>H \<^bold>{ M\<^sub>0 \<^bold>\<and> \<^bold>\<not> M\<^sub>1 \<^bold>} ((fst b) \<triangleright> do (snd b)) \<^bold>{ M\<^sub>1 \<^bold>}\<close>
+    proof -
+      let ?b = \<open>\<Pi>\<^sub>x!0\<close>
+      have \<open>\<turnstile>\<^sub>H \<^bold>{ M\<^sub>0 \<^bold>\<and> \<^bold>\<not> M\<^sub>1 \<^bold>} ((fst ?b) \<triangleright> do (snd ?b)) \<^bold>{ M\<^sub>1 \<^bold>}\<close>
+      proof 
+        show \<open>\<turnstile>\<^sub>H \<^bold>{ M\<^sub>0 \<^bold>\<and> \<^bold>\<not> M\<^sub>1 \<^bold>\<and> fst ?b \<^bold>} (snd ?b) \<^bold>{ M\<^sub>1 \<^bold>}\<close> sorry
+        show \<open>\<turnstile>\<^sub>M M\<^sub>0 \<^bold>\<and> \<^bold>\<not> M\<^sub>1 \<^bold>\<and> \<^bold>\<not> (fst ?b) \<^bold>\<longrightarrow> M\<^sub>1\<close> 
+        proof 
+          have \<open>\<Turnstile>\<^sub>P (M\<^sub>0 \<^bold>\<and> \<^bold>\<not> M\<^sub>1 \<^bold>\<and> \<^bold>\<not> (fst ?b) \<^bold>\<longrightarrow> M\<^sub>1)\<close> try
+          show \<open>\<turnstile>\<^sub>P M\<^sub>0 \<^bold>\<and> \<^bold>\<not> M\<^sub>1 \<^bold>\<and> \<^bold>\<not> (fst ?b) \<^bold>\<longrightarrow> M\<^sub>1\<close> sorry
+        qed
+      qed
+      then have \<open>\<Turnstile>\<^sub>H \<^bold>{ M\<^sub>0 \<^bold>\<and> \<^bold>\<not> M\<^sub>1 \<^bold>} ((fst ?b) \<triangleright> do (snd ?b)) \<^bold>{ M\<^sub>1 \<^bold>}\<close> using bw4t.soundness\<^sub>H by blast
+      then show ?thesis by auto
+    qed
+    ultimately have \<open>\<forall>s \<in> bw4t.Agent. \<forall>i. s, i \<Turnstile>\<^sub>T (M\<^sub>0\<^sup>T ensures M\<^sub>1\<^sup>T)\<close> using bw4t.ex_ensures by blast
+    then show ?thesis using bw4t.ensures by simp
+  qed    
+  moreover have \<open>\<dots> \<mapsto> M\<^sub>2\<^sup>T\<close>
+  proof -
+    have \<open>\<forall>b \<in> set \<Pi>\<^sub>x. (\<Turnstile>\<^sub>H \<^bold>{ M\<^sub>1 \<^bold>\<and> \<^bold>\<not> M\<^sub>2 \<^bold>} ((fst b) \<triangleright> do (snd b)) \<^bold>{ M\<^sub>1 \<^bold>\<or> M\<^sub>2 \<^bold>})\<close> sorry
+    moreover have \<open>\<exists>b \<in> set \<Pi>\<^sub>x. \<Turnstile>\<^sub>H \<^bold>{ M\<^sub>1 \<^bold>\<and> \<^bold>\<not> M\<^sub>2 \<^bold>} ((fst b) \<triangleright> do (snd b)) \<^bold>{ M\<^sub>2 \<^bold>}\<close> sorry
+    ultimately have \<open>\<forall>s \<in> bw4t.Agent. \<forall>i. s, i \<Turnstile>\<^sub>T (M\<^sub>1\<^sup>T ensures M\<^sub>2\<^sup>T)\<close> using bw4t.ex_ensures by blast
+    then show ?thesis using bw4t.ensures by simp
+  qed    
+  moreover have \<open>\<dots> \<mapsto> M\<^sub>3\<^sup>T\<close>
+  proof -
+    have \<open>\<forall>b \<in> set \<Pi>\<^sub>x. (\<Turnstile>\<^sub>H \<^bold>{ M\<^sub>2 \<^bold>\<and> \<^bold>\<not> M\<^sub>3 \<^bold>} ((fst b) \<triangleright> do (snd b)) \<^bold>{ M\<^sub>2 \<^bold>\<or> M\<^sub>3 \<^bold>})\<close> sorry
+    moreover have \<open>\<exists>b \<in> set \<Pi>\<^sub>x. \<Turnstile>\<^sub>H \<^bold>{ M\<^sub>2 \<^bold>\<and> \<^bold>\<not> M\<^sub>3 \<^bold>} ((fst b) \<triangleright> do (snd b)) \<^bold>{ M\<^sub>3 \<^bold>}\<close> sorry
+    ultimately have \<open>\<forall>s \<in> bw4t.Agent. \<forall>i. s, i \<Turnstile>\<^sub>T (M\<^sub>2\<^sup>T ensures M\<^sub>3\<^sup>T)\<close> using bw4t.ex_ensures by blast
+    then show ?thesis using bw4t.ensures by simp
+  qed    
+  moreover have \<open>\<dots> \<mapsto> M\<^sub>4\<^sup>T\<close>
+  proof -
+    have \<open>\<forall>b \<in> set \<Pi>\<^sub>x. (\<Turnstile>\<^sub>H \<^bold>{ M\<^sub>3 \<^bold>\<and> \<^bold>\<not> M\<^sub>4 \<^bold>} ((fst b) \<triangleright> do (snd b)) \<^bold>{ M\<^sub>3 \<^bold>\<or> M\<^sub>4 \<^bold>})\<close> sorry
+    moreover have \<open>\<exists>b \<in> set \<Pi>\<^sub>x. \<Turnstile>\<^sub>H \<^bold>{ M\<^sub>3 \<^bold>\<and> \<^bold>\<not> M\<^sub>4 \<^bold>} ((fst b) \<triangleright> do (snd b)) \<^bold>{ M\<^sub>4 \<^bold>}\<close> sorry
+    ultimately have \<open>\<forall>s \<in> bw4t.Agent. \<forall>i. s, i \<Turnstile>\<^sub>T (M\<^sub>3\<^sup>T ensures M\<^sub>4\<^sup>T)\<close> using bw4t.ex_ensures by blast
+    then show ?thesis using bw4t.ensures by simp
+  qed    
+  moreover have \<open>\<dots> \<mapsto> M\<^sub>5\<^sup>T\<close>
+  proof -
+    have \<open>\<forall>b \<in> set \<Pi>\<^sub>x. (\<Turnstile>\<^sub>H \<^bold>{ M\<^sub>4 \<^bold>\<and> \<^bold>\<not> M\<^sub>5 \<^bold>} ((fst b) \<triangleright> do (snd b)) \<^bold>{ M\<^sub>4 \<^bold>\<or> M\<^sub>5 \<^bold>})\<close> sorry
+    moreover have \<open>\<exists>b \<in> set \<Pi>\<^sub>x. \<Turnstile>\<^sub>H \<^bold>{ M\<^sub>4 \<^bold>\<and> \<^bold>\<not> M\<^sub>5 \<^bold>} ((fst b) \<triangleright> do (snd b)) \<^bold>{ M\<^sub>5 \<^bold>}\<close> sorry
+    ultimately have \<open>\<forall>s \<in> bw4t.Agent. \<forall>i. s, i \<Turnstile>\<^sub>T (M\<^sub>4\<^sup>T ensures M\<^sub>5\<^sup>T)\<close> using bw4t.ex_ensures by blast
+    then show ?thesis using bw4t.ensures by simp
+  qed    
+  ultimately show ?thesis using bw4t.imp by blast
+qed
+
+lemma \<open>s \<in> bw4t.Agent \<Longrightarrow> s, i \<Turnstile>\<^sub>T (M\<^sub>0\<^sup>T \<longrightarrow>\<^sub>T \<diamondop> (M\<^sub>5\<^sup>T))\<close>
+  using bw4t_lt bw4t.leads_to_temp by simp
 
 end
